Backup.

theories/common/bi_typeclasses.v
@@ -1,40 +1,17 @@
-From iris.bi Require Import
+From iris.bi Require Export
   bi.
+From iris.algebra Require Export
+  dfrac.
 From iris.proofmode Require Import
   proofmode.
 
-From tmc.common Require Import
+From simuliris.common Require Import
   prelude.
 
-Class BiEquiv (PROP : bi) X :=
-  bi_equiv : X → X → PROP.
-Infix "≈" := bi_equiv
-( at level 70,
-  no associativity
-) : bi_scope.
-Infix "≈@{ X }" := (@bi_equiv _ X _)
-( at level 70,
-  no associativity,
-  only parsing
-) : bi_scope.
-Notation "(≈)" := bi_equiv
-( only parsing
-) : bi_scope.
-Notation "(≈@{ X } )" := (@bi_equiv _ X _)
-( only parsing
-) : bi_scope.
-Notation "( x ≈.)" := (bi_equiv x)
-( only parsing
-) : bi_scope.
-Notation "(.≈ x )" := (λ y, bi_equiv y x)
-( only parsing
-) : bi_scope.
-
-Class BiWellFormed (PROP : bi) X :=
-  bi_well_formed : X → X → PROP.
+Implicit Types PROP : bi.
 
 Section Meet.
-  Context {PROP : bi}.
+  Context {PROP}.
 
   Global Instance bi_pred2_meet X1 X2 : Meet (X1 → X2 → PROP) := (
     λ Φ1 Φ2 x1 x2,
@@ -48,7 +25,7 @@ Section Meet.
 End Meet.
 
 Section Join.
-  Context {PROP : bi}.
+  Context {PROP}.
 
   Global Instance bi_pred2_join X1 X2 : Join (X1 → X2 → PROP) := (
     λ Φ1 Φ2 x1 x2,
@@ -76,14 +53,14 @@ Section Wand.
     λ Φ1 Φ2,
       ∀ x1 x2, Φ1 x1 x2 -∗ Φ2 x1 x2
   )%I.
-  Global Instance bi_pred2_wand_ne (X1 X2 : ofe) n
-  : Proper ((≡{n}≡) ==> (≡{n}≡) ==> (≡{n}≡)) $
+  Global Instance bi_pred2_wand_ne (X1 X2 : ofe) n :
+    Proper ((≡{n}≡) ==> (≡{n}≡) ==> (≡{n}≡)) $
     @wand (X1 -d> X2 -d> PROP) PROP _.
   Proof.
     rewrite /wand. solve_proper.
   Qed.
-  Global Instance bi_pred2_wand_proper (X1 X2 : ofe)
-  : Proper ((≡) ==> (≡) ==> (≡)) $
+  Global Instance bi_pred2_wand_proper (X1 X2 : ofe) :
+    Proper ((≡) ==> (≡) ==> (≡)) $
     @wand (X1 -d> X2 -d> PROP) PROP _.
   Proof.
     rewrite /wand. solve_proper.
@@ -93,16 +70,16 @@ Section Wand.
     λ Φ1 Φ2,
       ∀ x1 x2 x3, Φ1 x1 x2 x3 -∗ Φ2 x1 x2 x3
   )%I.
-  Global Instance bi_pred3_wand_ne (X1 X2 X3 : ofe) n
-  : Proper ((≡{n}≡) ==> (≡{n}≡) ==> (≡{n}≡)) $
+  Global Instance bi_pred3_wand_ne (X1 X2 X3 : ofe) n :
+    Proper ((≡{n}≡) ==> (≡{n}≡) ==> (≡{n}≡)) $
     @wand (X1 -d> X2 -d> X3 -d> PROP) PROP _.
   Proof.
     rewrite /wand /bi_pred3_wand.
     intros ? ? H1 ? ? H2.
     repeat (f_equiv || apply H1 || apply H2).
   Qed.
-  Global Instance bi_pred3_wand_proper (X1 X2 X3 : ofe)
-  : Proper ((≡) ==> (≡) ==> (≡)) $
+  Global Instance bi_pred3_wand_proper (X1 X2 X3 : ofe) :
+    Proper ((≡) ==> (≡) ==> (≡)) $
     @wand (X1 -d> X2 -d> X3 -d> PROP) PROP _.
   Proof.
     rewrite /wand /bi_pred3_wand.
@@ -118,14 +95,14 @@ Section BUpd.
     λ Φ x1 x2,
       |==> Φ x1 x2
   )%I.
-  Global Instance bi_pred2_bupd_ne (X1 X2 : ofe) n
-  : Proper ((≡{n}≡) ==> (≡{n}≡)) $
+  Global Instance bi_pred2_bupd_ne (X1 X2 : ofe) n :
+    Proper ((≡{n}≡) ==> (≡{n}≡)) $
     @bupd (X1 -d> X2 -d> PROP) _.
   Proof.
     rewrite /bupd. solve_proper.
   Qed.
-  Global Instance bi_pred2_bupd_proper (X1 X2 : ofe)
-  : Proper ((≡) ==> (≡)) $
+  Global Instance bi_pred2_bupd_proper (X1 X2 : ofe) :
+    Proper ((≡) ==> (≡)) $
     @bupd (X1 -d> X2 -d> PROP) _.
   Proof.
     rewrite /bupd. solve_proper.
@@ -140,16 +117,16 @@ Section BUpd.
     λ Φ x1 x2 x3,
       |==> Φ x1 x2 x3
   )%I.
-  Global Instance bi_pred3_bupd_ne (X1 X2 X3 : ofe) n
-  : Proper ((≡{n}≡) ==> (≡{n}≡)) $
+  Global Instance bi_pred3_bupd_ne (X1 X2 X3 : ofe) n :
+    Proper ((≡{n}≡) ==> (≡{n}≡)) $
     @bupd (X1 -d> X2 -d> X3 -d> PROP) _.
   Proof.
     rewrite /bupd /bi_pred3_bupd.
     intros ? ? H1 ? ? H2.
     repeat (f_equiv || apply H1 || apply H2).
   Qed.
-  Global Instance bi_pred3_bupd_proper (X1 X2 X3 : ofe)
-  : Proper ((≡) ==> (≡)) $
+  Global Instance bi_pred3_bupd_proper (X1 X2 X3 : ofe) :
+    Proper ((≡) ==> (≡)) $
     @bupd (X1 -d> X2 -d> X3 -d> PROP) _.
   Proof.
     rewrite /bupd /bi_pred3_bupd.
@@ -175,14 +152,14 @@ Notation "(===∗@{ X } )" := (λ Φ1 Φ2 : X, Φ1 ===∗ Φ2)%I
 Section WandBUpd.
   Context `{BiBUpd PROP}.
 
-  Global Instance bi_pred2_wand_bupd_ne (X1 X2 : ofe) n
-  : Proper ((≡{n}≡) ==> (≡{n}≡) ==> (≡{n}≡)) $
+  Global Instance bi_pred2_wand_bupd_ne (X1 X2 : ofe) n :
+    Proper ((≡{n}≡) ==> (≡{n}≡) ==> (≡{n}≡)) $
     (===∗@{X1 -d> X2 -d> PROP})%I.
   Proof.
     solve_proper.
   Qed.
-  Global Instance bi_pred2_wand_bupd_proper (X1 X2 : ofe)
-  : Proper ((≡) ==> (≡) ==> (≡)) $
+  Global Instance bi_pred2_wand_bupd_proper (X1 X2 : ofe) :
+    Proper ((≡) ==> (≡) ==> (≡)) $
     (===∗@{X1 -d> X2 -d> PROP})%I.
   Proof.
     solve_proper.
@@ -193,14 +170,14 @@ Section WandBUpd.
     iIntros "H" (? ?) "? !>". by iApply "H".
   Qed.
 
-  Global Instance bi_pred3_wand_bupd_ne (X1 X2 X3 : ofe) n
-  : Proper ((≡{n}≡) ==> (≡{n}≡) ==> (≡{n}≡)) $
+  Global Instance bi_pred3_wand_bupd_ne (X1 X2 X3 : ofe) n :
+    Proper ((≡{n}≡) ==> (≡{n}≡) ==> (≡{n}≡)) $
     (===∗@{X1 -d> X2 -d> X3 -d> PROP})%I.
   Proof.
     solve_proper.
   Qed.
-  Global Instance bi_pred3_wand_bupd_proper (X1 X2 X3 : ofe)
-  : Proper ((≡) ==> (≡) ==> (≡)) $
+  Global Instance bi_pred3_wand_bupd_proper (X1 X2 X3 : ofe) :
+    Proper ((≡) ==> (≡) ==> (≡)) $
     (===∗@{X1 -d> X2 -d> X3 -d> PROP})%I.
   Proof.
     solve_proper.
@@ -211,3 +188,307 @@ Section WandBUpd.
     iIntros "H" (? ? ?) "? !>". by iApply "H".
   Qed.
 End WandBUpd.
+
+Class BiSimilar PROP X Y :=
+  bi_similar : X → Y → PROP.
+Infix "≈" := bi_similar
+( at level 70,
+  no associativity
+) : bi_scope.
+Infix "{ X }@≈@{ Y }" := (@bi_similar _ X Y _)
+( at level 70,
+  no associativity,
+  only parsing
+) : bi_scope.
+Notation "(≈)" := bi_similar
+( only parsing
+) : bi_scope.
+Notation "({ X }@≈@{ Y } )" := (@bi_similar _ X Y _)
+( only parsing
+) : bi_scope.
+Notation "( x ≈.)" := (bi_similar x)
+( only parsing
+) : bi_scope.
+Notation "(.≈ y )" := (λ x, bi_similar x y)
+( only parsing
+) : bi_scope.
+
+Global Instance prod_bi_similar `{BiSimilar PROP X1 Y1} `{BiSimilar PROP X2 Y2}
+: BiSimilar PROP (X1 * X2) (Y1 * Y2)
+:= (
+  λ '(x1, x2) '(y1, y2),
+    x1 ≈ y1 ∗ x2 ≈ y2
+)%I.
+Global Instance prod_bi_similar_persistent
+  `{BiSimilar PROP X1 Y1} `{BiSimilar PROP X2 Y2}
+  `{∀ x1 y1, Persistent (x1 ≈ y1)} `{∀ x2 y2, Persistent (x2 ≈ y2)}
+  x1 x2 y1 y2 :
+    Persistent ((x1, x2) ≈ (y1, y2)).
+Proof.
+  apply _.
+Qed.
+
+Class BiPaired PROP X Y :=
+  bi_paired : X → Y → PROP.
+Infix "⟷" := bi_paired
+( at level 70,
+  no associativity
+) : bi_scope.
+Infix "{ X }@⟷@{ Y }" := (@bi_paired _ X Y _)
+( at level 70,
+  no associativity,
+  only parsing
+) : bi_scope.
+Notation "(⟷)" := bi_paired
+( only parsing
+) : bi_scope.
+Notation "({ X }@⟷@{ Y } )" := (@bi_paired _ X Y _)
+( only parsing
+) : bi_scope.
+Notation "( x ⟷.)" := (bi_paired x)
+( only parsing
+) : bi_scope.
+Notation "(.⟷ y )" := (λ x, bi_paired x y)
+( only parsing
+) : bi_scope.
+
+Global Instance prod_bi_paired `{BiPaired PROP X1 Y1} `{BiPaired PROP X2 Y2}
+: BiPaired PROP (X1 * X2) (Y1 * Y2)
+:= (
+  λ '(x1, x2) '(y1, y2),
+    x1 ⟷ y1 ∗ x2 ⟷ y2
+)%I.
+
+Class BiWellFormed PROP X :=
+  bi_well_formed : X → PROP.
+
+Class BiMapsto PROP loc val :=
+  bi_mapsto : loc → dfrac → val → PROP.
+Notation "l ↦{ dq } v" := (bi_mapsto l dq v)
+( at level 20,
+  format "l  ↦{ dq }  v"
+) : bi_scope.
+
+Class BiMapstoAny PROP loc :=
+  bi_mapsto_any : loc → dfrac → PROP.
+Notation "l ↦{ dq }-" := (bi_mapsto_any l dq)
+( at level 20,
+  format "l  ↦{ dq }-"
+) : bi_scope.
+Global Instance default_bi_mapsto_any `{BiMapsto PROP loc val}
+: BiMapstoAny PROP loc
+:= (λ l dq, ∃ v, l ↦{dq} v)%I.
+
+Class BiMapstoDiscarded PROP loc val :=
+  bi_mapsto_discarded : loc → val → PROP.
+Notation "l ↦□ v" := (bi_mapsto_discarded l v)
+( at level 20,
+  format "l  ↦□  v"
+) : bi_scope.
+Global Instance default_bi_mapsto_discarded `{BiMapsto PROP loc val}
+: BiMapstoDiscarded PROP loc val
+:= (λ l v, l ↦{DfracDiscarded} v)%I.
+
+Class BiMapstoDiscardedAny PROP loc :=
+  bi_mapsto_discarded_any : loc → PROP.
+Notation "l ↦□-" := (bi_mapsto_discarded_any l)
+( at level 20,
+  format "l  ↦□-"
+) : bi_scope.
+Global Instance default_bi_mapsto_discarded_any `{BiMapsto PROP loc val}
+: BiMapstoDiscardedAny PROP loc
+:= (λ l, ∃ v, l ↦□ v)%I.
+
+Class BiMapstoOwn PROP loc val :=
+  bi_mapsto_own : loc → Qp → val → PROP.
+Notation "l ↦{# q } v" := (bi_mapsto_own l q v)
+( at level 20,
+  format "l  ↦{# q }  v"
+) : bi_scope.
+Global Instance default_bi_mapsto_own `{BiMapsto PROP loc val}
+: BiMapstoOwn PROP loc val
+:= (λ l q v, l ↦{DfracOwn q} v)%I.
+
+Class BiMapstoOwnAny PROP loc :=
+  bi_mapsto_own_any : loc → Qp → PROP.
+Notation "l ↦{# q }-" := (bi_mapsto_own_any l q)
+( at level 20,
+  format "l  ↦{# q }-"
+) : bi_scope.
+Global Instance default_bi_mapsto_own_any `{BiMapsto PROP loc val}
+: BiMapstoOwnAny PROP loc
+:= (λ l q, ∃ v, l ↦{#q} v)%I.
+
+Class BiMapstoExcl PROP loc val :=
+  bi_mapsto_excl : loc → val → PROP.
+Notation "l ↦ v" := (bi_mapsto_excl l v)
+( at level 20,
+  format "l  ↦  v"
+) : bi_scope.
+Global Instance default_bi_mapsto_excl `{BiMapsto PROP loc val}
+: BiMapstoExcl PROP loc val
+:= (λ l v, l ↦{DfracOwn 1} v)%I.
+
+Class BiMapstoExclAny PROP loc :=
+  bi_mapsto_excl_any : loc → PROP.
+Notation "l ↦-" := (bi_mapsto_excl_any l)
+( at level 20,
+  format "l  ↦-"
+) : bi_scope.
+Global Instance default_bi_mapsto_excl_any `{BiMapsto PROP loc val}
+: BiMapstoExclAny PROP loc
+:= (λ l, ∃ v, l ↦ v)%I.
+
+Class BiMapstoₜ PROP loc val :=
+  bi_mapstoₜ : loc → dfrac → val → PROP.
+Notation "l ↦ₜ{ dq } v" := (bi_mapstoₜ l dq v)
+( at level 20,
+  format "l  ↦ₜ{ dq }  v"
+) : bi_scope.
+
+Class BiMapstoAnyₜ PROP loc :=
+  bi_mapsto_anyₜ : loc → dfrac → PROP.
+Notation "l ↦ₜ{ dq }-" := (bi_mapsto_anyₜ l dq)
+( at level 20,
+  format "l  ↦ₜ{ dq }-"
+) : bi_scope.
+Global Instance default_bi_mapsto_anyₜ `{BiMapstoₜ PROP loc val}
+: BiMapstoAnyₜ PROP loc
+:= (λ l dq, ∃ v, l ↦ₜ{dq} v)%I.
+
+Class BiMapstoDiscardedₜ PROP loc val :=
+  bi_mapsto_discardedₜ : loc → val → PROP.
+Notation "l ↦ₜ□ v" := (bi_mapsto_discardedₜ l v)
+( at level 20,
+  format "l  ↦ₜ□  v"
+) : bi_scope.
+Global Instance default_bi_mapsto_discardedₜ `{BiMapstoₜ PROP loc val}
+: BiMapstoDiscardedₜ PROP loc val
+:= (λ l v, l ↦ₜ{DfracDiscarded} v)%I.
+
+Class BiMapstoDiscardedAnyₜ PROP loc :=
+  bi_mapsto_discarded_anyₜ : loc → PROP.
+Notation "l ↦ₜ□-" := (bi_mapsto_discarded_anyₜ l)
+( at level 20,
+  format "l  ↦ₜ□-"
+) : bi_scope.
+Global Instance default_bi_mapsto_discarded_anyₜ `{BiMapstoₜ PROP loc val}
+: BiMapstoDiscardedAnyₜ PROP loc
+:= (λ l, ∃ v, l ↦ₜ□ v)%I.
+
+Class BiMapstoOwnₜ PROP loc val :=
+  bi_mapsto_ownₜ : loc → Qp → val → PROP.
+Notation "l ↦ₜ{# q } v" := (bi_mapsto_ownₜ l q v)
+( at level 20,
+  format "l  ↦ₜ{# q }  v"
+) : bi_scope.
+Global Instance default_bi_mapsto_ownₜ `{BiMapstoₜ PROP loc val}
+: BiMapstoOwnₜ PROP loc val
+:= (λ l q v, l ↦ₜ{DfracOwn q} v)%I.
+
+Class BiMapstoOwnAnyₜ PROP loc :=
+  bi_mapsto_own_anyₜ : loc → Qp → PROP.
+Notation "l ↦ₜ{# q }-" := (bi_mapsto_own_anyₜ l q)
+( at level 20,
+  format "l  ↦ₜ{# q }-"
+) : bi_scope.
+Global Instance default_bi_mapsto_own_anyₜ `{BiMapstoₜ PROP loc val}
+: BiMapstoOwnAnyₜ PROP loc
+:= (λ l q, ∃ v, l ↦ₜ{#q} v)%I.
+
+Class BiMapstoExclₜ PROP loc val :=
+  bi_mapsto_exclₜ : loc → val → PROP.
+Notation "l ↦ₜ v" := (bi_mapsto_exclₜ l v)
+( at level 20,
+  format "l  ↦ₜ  v"
+) : bi_scope.
+Global Instance default_bi_mapsto_exclₜ `{BiMapstoₜ PROP loc val}
+: BiMapstoExclₜ PROP loc val
+:= (λ l v, l ↦ₜ{DfracOwn 1} v)%I.
+
+Class BiMapstoExclAnyₜ PROP loc :=
+  bi_mapsto_excl_anyₜ : loc → PROP.
+Notation "l ↦ₜ-" := (bi_mapsto_excl_anyₜ l)
+( at level 20,
+  format "l  ↦ₜ-"
+) : bi_scope.
+Global Instance default_bi_mapsto_excl_anyₜ `{BiMapstoₜ PROP loc val}
+: BiMapstoExclAnyₜ PROP loc
+:= (λ l, ∃ v, l ↦ₜ v)%I.
+
+Class BiMapstoₛ PROP loc val :=
+  bi_mapstoₛ : loc → dfrac → val → PROP.
+Notation "l ↦ₛ{ dq } v" := (bi_mapstoₛ l dq v)
+( at level 20,
+  format "l  ↦ₛ{ dq }  v"
+) : bi_scope.
+
+Class BiMapstoAnyₛ PROP loc :=
+  bi_mapsto_anyₛ : loc → dfrac → PROP.
+Notation "l ↦ₛ{ dq }-" := (bi_mapsto_anyₛ l dq)
+( at level 20,
+  format "l  ↦ₛ{ dq }-"
+) : bi_scope.
+Global Instance default_bi_mapsto_anyₛ `{BiMapstoₛ PROP loc val}
+: BiMapstoAnyₛ PROP loc
+:= (λ l dq, ∃ v, l ↦ₛ{dq} v)%I.
+
+Class BiMapstoDiscardedₛ PROP loc val :=
+  bi_mapsto_discardedₛ : loc → val → PROP.
+Notation "l ↦ₛ□ v" := (bi_mapsto_discardedₛ l v)
+( at level 20,
+  format "l  ↦ₛ□  v"
+) : bi_scope.
+Global Instance default_bi_mapsto_discardedₛ `{BiMapstoₛ PROP loc val}
+: BiMapstoDiscardedₛ PROP loc val
+:= (λ l v, l ↦ₛ{DfracDiscarded} v)%I.
+
+Class BiMapstoDiscardedAnyₛ PROP loc :=
+  bi_mapsto_discarded_anyₛ : loc → PROP.
+Notation "l ↦ₛ□-" := (bi_mapsto_discarded_anyₛ l)
+( at level 20,
+  format "l  ↦ₛ□-"
+) : bi_scope.
+Global Instance default_bi_mapsto_discarded_anyₛ `{BiMapstoₛ PROP loc val}
+: BiMapstoDiscardedAnyₛ PROP loc
+:= (λ l, ∃ v, l ↦ₛ□ v)%I.
+
+Class BiMapstoOwnₛ PROP loc val :=
+  bi_mapsto_ownₛ : loc → Qp → val → PROP.
+Notation "l ↦ₛ{# q } v" := (bi_mapsto_ownₛ l q v)
+( at level 20,
+  format "l  ↦ₛ{# q }  v"
+) : bi_scope.
+Global Instance default_bi_mapsto_ownₛ `{BiMapstoₛ PROP loc val}
+: BiMapstoOwnₛ PROP loc val
+:= (λ l q v, l ↦ₛ{DfracOwn q} v)%I.
+
+Class BiMapstoOwnAnyₛ PROP loc :=
+  bi_mapsto_own_anyₛ : loc → Qp → PROP.
+Notation "l ↦ₛ{# q }-" := (bi_mapsto_own_anyₛ l q)
+( at level 20,
+  format "l  ↦ₛ{# q }-"
+) : bi_scope.
+Global Instance default_bi_mapsto_own_anyₛ `{BiMapstoₛ PROP loc val}
+: BiMapstoOwnAnyₛ PROP loc
+:= (λ l q, ∃ v, l ↦ₛ{#q} v)%I.
+
+Class BiMapstoExclₛ PROP loc val :=
+  bi_mapsto_exclₛ : loc → val → PROP.
+Notation "l ↦ₛ v" := (bi_mapsto_exclₛ l v)
+( at level 20,
+  format "l  ↦ₛ  v"
+) : bi_scope.
+Global Instance default_bi_mapsto_exclₛ `{BiMapstoₛ PROP loc val}
+: BiMapstoExclₛ PROP loc val
+:= (λ l v, l ↦ₛ{DfracOwn 1} v)%I.
+
+Class BiMapstoExclAnyₛ PROP loc :=
+  bi_mapsto_excl_anyₛ : loc → PROP.
+Notation "l ↦ₛ-" := (bi_mapsto_excl_anyₛ l)
+( at level 20,
+  format "l  ↦ₛ-"
+) : bi_scope.
+Global Instance default_bi_mapsto_excl_anyₛ `{BiMapstoₛ PROP loc val}
+: BiMapstoExclAnyₛ PROP loc
+:= (λ l, ∃ v, l ↦ₛ v)%I.
