theories/common/loc.v
@@ -1,65 +1,73 @@
+From stdpp Require Import
+  countable
+  infinite
+  gmap.
+
 From iris.algebra Require Import
   ofe.
 
-From stdpp Require Import
-  countable
-  numbers
-  gmap.
-
-From tmc.common Require Import
+From simuliris.common Require Import
   prelude.
 
-Record loc := { loc_car : Z }.
+(* ---------- block ---------- *)
 
-Canonical Structure locO := leibnizO loc.
+Definition block := positive.
 
-Global Instance loc_eq_decision : EqDecision loc.
+(* ---------- index ---------- *)
+
+Inductive index := one | two.
+
+Global Instance index_pair_lookup_total X : LookupTotal index X (X * X) :=
+  λ i p,
+    match i with
+    | one => p.1
+    | two => p.2
+    end.
+
+Global Instance index_eq_dec :
+  EqDecision index.
 Proof.
   solve_decision.
 Qed.
-Global Instance loc_inhabited : Inhabited loc :=
-  populate {| loc_car := 0 |}.
-Global Instance loc_countable : Countable loc.
+Global Instance index_inhabited : Inhabited index :=
+  populate one.
+Global Instance index_countable :
+  Countable index.
 Proof.
-  by apply (inj_countable' loc_car (λ i, {| loc_car := i |})); intros [].
-Qed.
-Program Global Instance loc_infinite : Infinite loc :=
-  inj_infinite (λ p, {| loc_car := p |}) (λ l, Some (loc_car l)) _.
-Next Obligation.
-  done.
+  apply (
+    inj_countable (
+      λ i,
+        match i with
+        | one => true
+        | two => false
+        end
+    ) (
+      λ n,
+        match n with
+        | true => Some one
+        | false => Some two
+        end
+    )
+  ).
+  intros []; eauto.
 Qed.
 
-Definition loc_add l off :=
-  {| loc_car := loc_car l + off |}.
-Infix "+ₗ" := loc_add
-( at level 50,
-  left associativity
-) : stdpp_scope.
+(* ---------- loc ---------- *)
 
-Lemma loc_add_assoc l i j :
-  l +ₗ i +ₗ j = l +ₗ (i + j).
+Definition loc : Type := block * index.
+
+Global Instance block_locset_elem_of : ElemOf block (gset loc) :=
+  λ blk locs,
+    ∃ i, (blk, i) ∈ locs.
+
+Global Instance block_locset_fresh : Fresh block (gset loc) :=
+  λ locs,
+    fresh (elements locs).*1.
+Lemma block_locset_fresh_spec (locs : gset loc) :
+  fresh locs ∉ locs.
 Proof.
-  destruct l; rewrite /loc_add /=; f_equal; lia.
-Qed.
-Lemma loc_add_0 l :
-  l +ₗ 0 = l.
-Proof.
-  destruct l; rewrite /loc_add /=; f_equal; lia.
-Qed.
-Global Instance loc_add_inj l : Inj eq eq (loc_add l).
-Proof.
-  destruct l; rewrite /Inj /loc_add /=; intros; simplify_eq; lia.
+  intros [i ?%elem_of_elements%(elem_of_list_fmap_1 fst)].
+  eapply infinite_is_fresh. eauto.
 Qed.
 
-Definition loc_fresh (locs : gset loc) : loc :=
-  {| loc_car := set_fold (λ k r, (1 + loc_car k) `max` r)%Z 1%Z locs |}.
-Global Opaque loc_fresh.
-
-Lemma loc_fresh_spec locs i :
-  (0 ≤ i)%Z → loc_fresh locs +ₗ i ∉ locs.
-Proof.
-  intros Hi. cut (∀ l, l ∈ locs → loc_car l < loc_car (loc_fresh locs) + i)%Z.
-  { intros help Hf%help. simpl in *. lia. }
-  apply (set_fold_ind_L (λ r ls, ∀ l, l ∈ ls → (loc_car l < r + i)%Z));
-    set_solver by eauto with lia.
-Qed.
+Canonical locO := leibnizO loc.
