theories/common/typeclasses.v
@@ -1,5 +1,94 @@
-From tmc.common Require Import
+From simuliris.common Require Import
   prelude.
+
+Class SqSubset X :=
+  sqsubset : relation X.
+Infix "⊏" := sqsubset
+( at level 70
+) : stdpp_scope.
+Infix "⊏@{ X }" := (@sqsubset X _)
+( at level 70,
+  only parsing
+) : stdpp_scope.
+Notation "(⊏)" := sqsubset
+( only parsing
+) : stdpp_scope.
+Notation "(⊏@{ X } )" := (@sqsubset X _)
+( only parsing
+) : stdpp_scope.
+Notation "( x ⊏.)" := (sqsubset x)
+( only parsing
+) : stdpp_scope.
+Notation "(.⊏ y )" := (λ x, sqsubset x y)
+( only parsing
+) : stdpp_scope.
+
+Class Similar X Y :=
+  similar : X → Y → Prop.
+Infix "≈" := similar
+( at level 70,
+  no associativity
+) : stdpp_scope.
+Infix "{ X }@≈@{ Y }" := (@similar X Y _)
+( at level 70,
+  no associativity,
+  only parsing
+) : stdpp_scope.
+Notation "(≈)" := similar
+( only parsing
+) : stdpp_scope.
+Notation "({ X }@≈@{ Y } )" := (@similar X Y _)
+( only parsing
+) : stdpp_scope.
+Notation "( x ≈.)" := (similar x)
+( only parsing
+) : stdpp_scope.
+Notation "(.≈ y )" := (λ x, similar x y)
+( only parsing
+) : stdpp_scope.
+
+Class Refines X Y :=
+  refines : X → Y → Prop.
+Infix "⊴" := refines
+( at level 70,
+  no associativity
+) : stdpp_scope.
+Infix "{ X }@⊴@{ Y }" := (@refines X Y _)
+( at level 70,
+  no associativity,
+  only parsing
+) : stdpp_scope.
+Notation "(⊴)" := refines
+( only parsing
+) : stdpp_scope.
+Notation "({ X }@⊴@{ Y } )" := (@refines X Y _)
+( only parsing
+) : stdpp_scope.
+Notation "( x ⊴.)" := (refines x)
+( only parsing
+) : stdpp_scope.
+Notation "(.⊴ y )" := (λ x, refines x y)
+( only parsing
+) : stdpp_scope.
 
 Class WellFormed X :=
   well_formed : X → Prop.
+
+Class Closed X :=
+  closed : X → Prop.
+
+Class Fill ctx expr :=
+  fill : ctx → expr → expr.
+Global Arguments fill {_ _ _} _ _ : assert.
+Notation "C @@ e" := (fill C e)
+( at level 20
+) : stdpp_scope.
+Notation "(@@)" := fill
+( only parsing
+) : stdpp_scope.
+Notation "( C @@.)" := (fill C)
+( only parsing
+) : stdpp_scope.
+Notation "(.@@ e )" := (λ C, fill C e)
+( only parsing
+) : stdpp_scope.
