theories/without_calls/refinement.v
@@ -1,48 +1,59 @@
-From tmc.common Require Export
-  prelude.
-From tmc.without_calls.language Require Export
-  lang.
+From simuliris.common Require Import
+  prelude
+  typeclasses.
+From simuliris.without_calls Require Export
+  lang.lang.
 
 Section behaviour.
   Context {Λ : lang}.
 
   Inductive behaviour :=
-    | behaviour_converge : expr Λ → behaviour
-    | behaviour_diverge : behaviour.
+    | behaviour_converges : expr Λ → behaviour
+    | behaviour_diverges : behaviour.
 
   Inductive has_behaviour e σ : behaviour → Prop :=
-    | has_behaviour_converge e' σ' :
-        rtc step (e, σ) (e', σ') →
-        irreducible e' σ' →
-        has_behaviour e σ (behaviour_converge e')
-    | has_behaviour_diverge :
-        diverge e σ →
-        has_behaviour e σ behaviour_diverge.
-
-  Section behaviour_refinement.
-    Context `{Equiv (val Λ)}.
-
-    Inductive behaviour_refinement : SqSubsetEq behaviour :=
-      | behaviour_refinement_val eₜ vₜ eₛ vₛ :
-          eₜ = of_val vₜ →
-          eₛ = of_val vₛ →
-          vₜ ≡ vₛ →
-          behaviour_refinement (behaviour_converge eₜ) (behaviour_converge eₛ)
-      | behaviour_refinement_stuck eₜ eₛ :
-          to_val eₜ = None →
-          to_val eₛ = None →
-          behaviour_refinement (behaviour_converge eₜ) (behaviour_converge eₛ)
-      | behaviour_refinement_diverge :
-          behaviour_refinement behaviour_diverge behaviour_diverge.
-    Global Existing Instance behaviour_refinement.
-
-    Lemma behaviour_refinement_strongly_stuck eₜ eₛ :
-      strongly_stuck eₜ →
-      strongly_stuck eₛ →
-      behaviour_converge eₜ ⊑ behaviour_converge eₛ.
-    Proof.
-      rewrite /strongly_stuck. intros.
-      apply behaviour_refinement_stuck; naive_solver.
-    Qed.
-  End behaviour_refinement.
+    | has_behaviour_converges e' σ' :
+        converges e σ e' σ' →
+        has_behaviour e σ (behaviour_converges e')
+    | has_behaviour_diverges :
+        diverges e σ →
+        has_behaviour e σ behaviour_diverges.
 End behaviour.
+Global Arguments behaviour : clear implicits.
+
+Section refinement.
+  Context `{Similar (val Λₜ) (val Λₛ)}.
+
+  Inductive behaviour_refinement : Refines (behaviour Λₜ) (behaviour Λₛ) :=
+    | behaviour_refinement_val eₜ vₜ eₛ vₛ :
+        eₜ = of_val vₜ →
+        eₛ = of_val vₛ →
+        vₜ ≈ vₛ →
+        behaviour_refinement (behaviour_converges eₜ) (behaviour_converges eₛ)
+    | behaviour_refinement_stuck eₜ eₛ :
+        to_val eₜ = None →
+        to_val eₛ = None →
+        behaviour_refinement (behaviour_converges eₜ) (behaviour_converges eₛ)
+    | behaviour_refinement_diverges :
+        behaviour_refinement behaviour_diverges behaviour_diverges.
+  Global Existing Instance behaviour_refinement.
+
+  Global Instance refinement : Refines (cfg Λₜ) (cfg Λₛ) :=
+    λ '(eₜ, σₜ) '(eₛ, σₛ),
+      ∀ bₜ, has_behaviour eₜ σₜ bₜ →
+      ∃ bₛ, has_behaviour eₛ σₛ bₛ ∧ bₜ ⊴ bₛ.
+End refinement.
+
+Section crefinement.
+  Context {Λ : lang}.
+  Context (ctx : Type).
+  Context `{Similar (val Λ) (val Λ)} `{Closed (expr Λ)} `{Empty (state Λ)}.
+  Context `{LangCtx Λ ctx} `{WellFormed ctx}.
+
+  Global Instance crefinement : Refines (expr Λ) (expr Λ) :=
+    λ eₜ eₛ,
+      ∀ C, well_formed C →
+      closed (C @@ eₜ) →
+      closed (C @@ eₛ) →
+      (C @@ eₜ, ∅) ⊴ (C @@ eₛ, ∅).
+End crefinement.
