theories/common/relations.v
@@ -1,0 +1,24 @@
+From simuliris.common Require Import
+  prelude.
+
+Section relation.
+  Context `{R : relation X}.
+
+  Lemma Acc_tc x :
+    Acc R x →
+    Acc (tc R) x.
+  Proof.
+    intros Hx. induction Hx. econstructor.
+    intros y Hy. induction Hy.
+    - eauto.
+    - eapply Acc_inv.
+      + eapply IHHy; done.
+      + eauto using tc_once.
+  Qed.
+  Lemma tc_wf :
+    wf R →
+    wf (tc R).
+  Proof.
+    intros ? ?**. eauto using Acc_tc.
+  Qed.
+End relation.
