theories/common/simul_heap_bij.v
@@ -1,0 +1,149 @@
+From iris.base_logic.lib Require Import
+  gset_bij.
+From iris.base_logic.lib Require Export
+  iprop.
+From iris.proofmode Require Import
+  proofmode.
+
+From simuliris.common Require Export
+  bi_typeclasses
+  simul_heap.
+
+Class SimulHeapBijGpreS locₜ locₛ valₜ valₛ Σ `{SimulHeapGS locₜ locₛ valₜ valₛ Σ} :=
+  simul_heap_bij_GpreS_bij_G : gset_bijG Σ locₜ locₛ.
+Local Existing Instance simul_heap_bij_GpreS_bij_G.
+
+Class SimulHeapBijGS locₜ locₛ valₜ valₛ Σ `{SimulHeapGS locₜ locₛ valₜ valₛ Σ} := {
+  simul_heap_bij_GS_bij_G : gset_bijG Σ locₜ locₛ ;
+  simul_heap_bij_GS_name : gname ;
+}.
+Arguments Build_SimulHeapBijGS locₜ locₛ valₜ valₛ Σ {_ _ _ _ _ _} _: assert.
+Arguments simul_heap_bij_GS_name {_ _ _ _ _ _ _ _ _ _ _} : assert.
+Local Existing Instance simul_heap_bij_GS_bij_G.
+
+Section simul_heap_bij.
+  Context `{SimulHeapBijGS locₜ locₛ valₜ valₛ Σ}.
+  Implicit Types lₜ : locₜ.
+  Implicit Types lₛ : locₛ.
+  Implicit Types vₜ : valₜ.
+  Implicit Types vₛ : valₛ.
+
+  Definition simul_heap_bij_auth (bij : gset (locₜ * locₛ)) :=
+    gset_bij_own_auth simul_heap_bij_GS_name (DfracOwn 1) bij.
+
+  Definition simul_heap_bij_elem lₜ lₛ :=
+    gset_bij_own_elem simul_heap_bij_GS_name lₜ lₛ.
+  Global Instance loc_bi_similar : BiSimilar _ locₜ locₛ :=
+    simul_heap_bij_elem.
+
+  Global Instance simul_heap_bij_elem_persistent lₜ lₛ :
+    Persistent (lₜ ≈ lₛ).
+  Proof.
+    apply _.
+  Qed.
+
+  Lemma simul_heap_bij_agree lₜ1 lₜ2 lₛ1 lₛ2 :
+    lₜ1 ≈ lₛ1 -∗
+    lₜ2 ≈ lₛ2 -∗
+    ⌜lₜ1 = lₜ2 ↔ lₛ1 = lₛ2⌝.
+  Proof.
+    iIntros "H1 H2". iApply (gset_bij_own_elem_agree with "H1 H2").
+  Qed.
+  Lemma simul_heap_bij_func lₜ lₛ1 lₛ2 :
+    lₜ ≈ lₛ1 -∗
+    lₜ ≈ lₛ2 -∗
+    ⌜lₛ1 = lₛ2⌝.
+  Proof.
+    iIntros "H1 H2". iPoseProof (simul_heap_bij_agree with "H1 H2") as "<-"; done.
+  Qed.
+  Lemma simul_heap_bij_inj lₛ lₜ1 lₜ2 :
+    lₜ1 ≈ lₛ -∗
+    lₜ2 ≈ lₛ -∗
+    ⌜lₜ1 = lₜ2⌝.
+  Proof.
+    iIntros "H1 H2". iPoseProof (simul_heap_bij_agree with "H1 H2") as "->"; done.
+  Qed.
+
+  Section val_similar.
+    Context `{BiSimilar (iPropI Σ) valₜ valₛ}.
+
+    Global Instance loc_bi_paired : BiPaired _ locₜ locₛ := (
+      λ lₜ lₛ,
+        ∃ vₜ vₛ,
+        lₜ ↦ₜ vₜ ∗ lₛ ↦ₛ vₛ ∗ vₜ ≈ vₛ
+    )%I.
+
+    Definition simul_heap_bij_inv := (
+      ∃ bij,
+      simul_heap_bij_auth bij ∗
+      [∗ set] p ∈ bij, p.1 ⟷ p.2
+    )%I.
+
+    Lemma simul_heap_bij_access lₜ lₛ :
+      simul_heap_bij_inv -∗
+      lₜ ≈ lₛ -∗
+      lₜ ⟷ lₛ ∗ (lₜ ⟷ lₛ -∗ simul_heap_bij_inv).
+    Proof.
+      iIntros "(% & Hauth & Hpairing) #Hsimil".
+      iDestruct (gset_bij_elem_of with "[$] [$]") as "%".
+      iDestruct (big_sepS_delete with "Hpairing") as "(Hpaired & ?)"; first done.
+      iDestruct "Hpaired" as "(% & % & Hpaired)".
+      iSplitL "Hpaired"; first by repeat iExists _.
+      iIntros. iExists _. iFrame "Hauth".
+      iApply big_sepS_delete; [done | by iFrame].
+    Qed.
+
+    Lemma simul_heap_bij_insert lₜ lₛ :
+      simul_heap_bij_inv -∗
+      lₜ ⟷ lₛ ==∗
+      simul_heap_bij_inv ∗ lₜ ≈ lₛ.
+    Proof.
+      iIntros "Hinv (%vₜ & %vₛ & Ht & Hs & Hrel)".
+      iDestruct "Hinv" as (bij) "[Hauth Hheap]".
+      iAssert ((¬ ⌜set_Exists (λ '(lₜ', lₛ'), lₜ = lₜ') bij⌝)%I) as "%Hextₜ".
+      { iIntros (([lₜ' lₛ'] & Hin & <-)).
+        iPoseProof (big_sepS_elem_of with "Hheap") as (vₜ' vₛ') "(Hcon & _ & _)".
+        { eapply Hin. }
+        iPoseProof (simul_mapstoₜ_valid_2  with "Ht Hcon") as "%Hcon"; exfalso.
+        destruct Hcon as [Hcon _]. by apply dfrac_valid_own_r in Hcon.
+      }
+      iAssert ((¬ ⌜set_Exists (λ '(lₜ', lₛ'), lₛ = lₛ') bij⌝)%I) as "%Hextₛ".
+      { iIntros (([lₜ' lₛ'] & Hin & <-)).
+        iPoseProof (big_sepS_elem_of with "Hheap") as (vₜ' vₛ') "(_ & Hcon & _)".
+        { eapply Hin. }
+        iPoseProof (simul_mapstoₛ_valid_2 with "Hs Hcon") as "%Hcon"; exfalso.
+        destruct Hcon as [Hcon _]. by apply dfrac_valid_own_r in Hcon.
+      }
+      iMod ((gset_bij_own_extend lₜ lₛ) with "Hauth") as "[Hinv #Helem]".
+      - intros lₛ' Hlₛ'. apply Hextₜ. by exists (lₜ, lₛ').
+      - intros lₜ' Hlₜ'. apply Hextₛ. by exists (lₜ', lₛ).
+      - iModIntro. iSplitL; last done.
+        iExists _. iFrame.
+        iApply big_sepS_insert. { contradict Hextₜ. by exists (lₜ, lₛ). }
+        iFrame. iExists vₜ, vₛ. iFrame.
+    Qed.
+  End val_similar.
+End simul_heap_bij.
+
+Section init.
+  Context `{SimulHeapBijGpreS locₜ locₛ valₜ valₛ Σ}.
+  Context `{BiSimilar (iPropI Σ) valₜ valₛ}.
+
+  Lemma simul_heap_bij_init_names :
+    ⊢ |==> ∃ γ : gname,
+      let _ := Build_SimulHeapBijGS locₜ locₛ valₜ valₛ Σ γ in
+      simul_heap_bij_inv.
+  Proof.
+    iMod (gset_bij_own_alloc_empty) as (γ) "Hinv".
+    iExists γ. iModIntro. iExists (∅). iSplitL "Hinv"; first by iApply "Hinv".
+    by iApply big_sepS_empty.
+  Qed.
+
+  Lemma simul_heap_bij_init :
+    ⊢ |==> ∃ _ : SimulHeapBijGS locₜ locₛ valₜ valₛ Σ,
+      simul_heap_bij_inv.
+  Proof.
+    iMod (simul_heap_bij_init_names) as (γ) "Hinit".
+    iModIntro. iExists (Build_SimulHeapBijGS _ _ _ _ _ γ). iFrame.
+  Qed.
+End init.
