theories/common/tactics.v
@@ -1,13 +1,11 @@
 From Coq.Program Require Import
   Tactics.
 
-From tmc.common Require Import
+From simuliris.common Require Import
   prelude.
 
-Ltac invert H :=
-  inversion_clear H; simplify_eq.
-Ltac simple_invert H :=
-  simple inversion H; clear H; simplify_eq.
-
 Ltac simplify :=
-  program_simplify.
+  program_simplify; simplify_eq/=.
+
+Ltac invert H :=
+  inversion H; clear H; simplify_eq/=.
