theories/without_calls/lang/ectx_lang.v
@@ -1,0 +1,333 @@
+From simuliris.common Require Import
+  prelude
+  tactics.
+From simuliris.without_calls Require Export
+  lang.lang.
+
+Section LangEctxMixin.
+  Context {val expr state : Type}.
+  Context (to_val : expr → option val).
+  Context (head_step : expr → state → expr → state → Prop).
+  Context (ectx : Type) `{LangCtxBase expr ectx}.
+  Implicit Types e : expr.
+  Implicit Types K : ectx.
+
+  Record LangEctxMixin := {
+    lang_ectx_mixin_ctx_mixin :
+      LangCtxMixin to_val ectx ;
+    lang_ectx_mixin_fill_redex K K_redex e1 e1_redex σ1 e2 σ2 :
+      K @@ e1 = K_redex @@ e1_redex →
+      to_val e1 = None →
+      head_step e1_redex σ1 e2 σ2 →
+      ∃ K', K_redex = K ⋅ K' ;
+    lang_ectx_mixin_fill_head_step_val K e1 σ1 e2 σ2 :
+      head_step (K @@ e1) σ1 e2 σ2 →
+      is_Some (to_val e1) ∨ K = ∅ ;
+  }.
+End LangEctxMixin.
+Global Arguments Build_LangEctxMixin {_ _ _ _ _ _ _} _ _ _ : assert.
+
+Section EctxLangMixin.
+  Context {expr val state : Type}.
+  Context (of_val : val → expr).
+  Context (to_val : expr → option val).
+  Context (head_step : expr → state → expr → state → Prop).
+  Context (ectx : Type) `{LangCtxBase expr ectx}.
+
+  Record EctxLangMixin := {
+    ectx_lang_mixin_to_of_val e v :
+      e = of_val v →
+      to_val e = Some v ;
+    ectx_lang_mixin_of_to_val e v :
+      to_val e = Some v →
+      of_val v = e ;
+    ectx_lang_mixin_head_step_not_val e1 σ1 e2 σ2 :
+      head_step e1 σ1 e2 σ2 →
+      to_val e1 = None ;
+    ectx_lang_mixin_ectx_mixin :
+      LangEctxMixin to_val head_step ectx ;
+  }.
+End EctxLangMixin.
+Global Arguments Build_EctxLangMixin {_ _ _ _ _ _ _ _} _ _ _ _ : assert.
+
+Structure ectx_lang := {
+  expr : Type ;
+  val : Type ;
+  state : Type ;
+  of_val : val → expr ;
+  to_val : expr → option val ;
+  head_step : expr → state → expr → state → Prop ;
+  ectx : Type ;
+  ectx_lang_ctx_base : LangCtxBase expr ectx ;
+  ectx_lang_mixin : EctxLangMixin of_val to_val head_step ectx ;
+}.
+Global Arguments Build_ectx_lang {_ _ _ _ _ _ _ _} _ : assert.
+Global Arguments of_val {_} _ : assert.
+Global Arguments to_val {_} _ : assert.
+Global Arguments head_step {_} _ _ _ _ : assert.
+Global Existing Instance ectx_lang_ctx_base.
+
+Section ectx_lang.
+  Context {Λ : ectx_lang}.
+  Implicit Types v : val Λ.
+  Implicit Types e : expr Λ.
+  Implicit Types K : ectx Λ.
+
+  Inductive prim_step e1 σ1 e2 σ2 : Prop :=
+    | head_step_fill_prim_step K e1' e2' :
+        e1 = K @@ e1' →
+        e2 = K @@ e2' →
+        head_step e1' σ1 e2' σ2 →
+        prim_step e1 σ1 e2 σ2.
+  Hint Constructors prim_step : core.
+
+  Definition head_reducible e σ :=
+    ∃ e' σ', head_step e σ e' σ'.
+  Definition head_irreducible e σ :=
+    ∀ e' σ', ¬ head_step e σ e' σ'.
+  Definition head_stuck e σ :=
+    to_val e = None ∧ head_irreducible e σ.
+
+  Definition sub_redexes_are_values e :=
+    ∀ K e',
+    e = K @@ e' →
+    to_val e' = None →
+    K = ∅.
+
+  Class StronglyHeadReducible e :=
+    strongly_head_reducible σ : head_reducible e σ.
+  Class StronglyHeadIrreducible e :=
+    strongly_head_irreducible σ : head_irreducible e σ.
+  Class StronglyHeadStuck e := {
+    strongly_head_stuck_strongly_head_irreducible :> StronglyHeadIrreducible e ;
+    strongly_head_stuck_not_val : to_val e = None ;
+    strongly_head_stuck_sub_redexes_are_values : sub_redexes_are_values e ;
+  }.
+
+  Record pure_head_step e1 e2 := {
+    pure_head_step_safe σ1 :
+      head_reducible e1 σ1 ;
+    pure_head_step_det σ1 e2' σ2 :
+      head_step e1 σ1 e2' σ2 →
+      σ2 = σ1 ∧ e2' = e2 ;
+  }.
+  Class PureHeadExec (ϕ : Prop) n e1 e2 :=
+    pure_head_exec : ϕ → nsteps pure_head_step n e1 e2.
+
+  Lemma head_step_not_val e1 σ1 e2 σ2 :
+    head_step e1 σ1 e2 σ2 →
+    to_val e1 = None.
+  Proof.
+    apply ectx_lang_mixin.
+  Qed.
+  Lemma fill_empty e :
+    ∅ @@ e = e.
+  Proof.
+    apply ectx_lang_mixin.
+  Qed.
+  Lemma fill_op K1 K2 e :
+    K1 @@ (K2 @@ e) = (K1 ⋅ K2) @@ e.
+  Proof.
+    apply ectx_lang_mixin.
+  Qed.
+  Global Instance fill_inj K :
+    Inj (=) (=) (K @@.).
+  Proof.
+    apply ectx_lang_mixin.
+  Qed.
+  Lemma fill_not_val K e :
+    to_val e = None →
+    to_val (K @@ e) = None.
+  Proof.
+    apply ectx_lang_mixin.
+  Qed.
+  Lemma fill_redex K K_redex e1 e1_redex σ1 e2 σ2 :
+    K @@ e1 = K_redex @@ e1_redex →
+    to_val e1 = None →
+    head_step e1_redex σ1 e2 σ2 →
+    ∃ K', K_redex = K ⋅ K'.
+  Proof.
+    apply ectx_lang_mixin.
+  Qed.
+  Lemma fill_head_step_val K e σ1 e2 σ2 :
+    head_step (K @@ e) σ1 e2 σ2 →
+    is_Some (to_val e) ∨ K = ∅.
+  Proof.
+    apply ectx_lang_mixin.
+  Qed.
+
+  Lemma lang_of_ectx_lang_mixin :
+    LangMixin of_val to_val prim_step.
+  Proof.
+    constructor.
+    - apply ectx_lang_mixin.
+    - apply ectx_lang_mixin.
+    - intros * [? ? ? -> -> ?%head_step_not_val]. eapply fill_not_val. done.
+  Qed.
+  Canonical lang_of_ectx_lang' := Build_lang lang_of_ectx_lang_mixin.
+
+  Lemma head_step_prim_step e1 σ1 e2 σ2 :
+    head_step e1 σ1 e2 σ2 →
+    prim_step e1 σ1 e2 σ2.
+  Proof.
+    econstructor; eauto using fill_empty.
+  Qed.
+  Lemma prim_step_fill_prim_step K e1 σ1 e2 σ2 :
+    prim_step e1 σ1 e2 σ2 →
+    prim_step (K @@ e1) σ1 (K @@ e2) σ2.
+  Proof.
+    intros []. simplify. eauto using fill_op.
+  Qed.
+
+  Lemma head_irreducible_not_head_reducible e σ :
+    head_irreducible e σ ↔
+    ¬ head_reducible e σ.
+  Proof.
+    rewrite /head_reducible /head_irreducible. naive_solver.
+  Qed.
+  Lemma reducible_fill_reducible K e σ :
+    reducible e σ →
+    reducible (K @@ e) σ.
+  Proof.
+    intros (? & ? & ?). do 2 eexists. eapply prim_step_fill_prim_step. eauto.
+  Qed.
+  Lemma head_reducible_fill_reducible K e σ :
+    head_reducible e σ →
+    reducible (K @@ e) σ.
+  Proof.
+    intros (? & ? & ?). do 2 eexists. eapply head_step_fill_prim_step; eauto.
+  Qed.
+  Lemma head_reducible_reducible e σ :
+    head_reducible e σ →
+    reducible e σ.
+  Proof.
+    rewrite -{2}(fill_empty e). eauto using head_reducible_fill_reducible.
+  Qed.
+  Lemma reducible_head_reducible e σ :
+    reducible e σ →
+    sub_redexes_are_values e →
+    head_reducible e σ.
+  Proof.
+    intros (? & ? & []) ?. simplify.
+    assert (K = ∅) as -> by eauto using head_step_not_val.
+    rewrite fill_empty /head_reducible; eauto.
+  Qed.
+  Lemma head_irreducible_irreducible e σ :
+    head_irreducible e σ →
+    sub_redexes_are_values e →
+    irreducible e σ.
+  Proof.
+    rewrite irreducible_not_reducible head_irreducible_not_head_reducible.
+    eauto using reducible_head_reducible.
+  Qed.
+  Lemma head_reducible_fill_prim_step K e1 σ1 e2 σ2 :
+    head_reducible e1 σ1 →
+    prim_step (K @@ e1) σ1 e2 σ2 →
+    ∃ e2', e2 = K @@ e2' ∧ head_step e1 σ1 e2' σ2.
+  Proof.
+    intros (? & ? & Hstep) [K' e1' e2' Heq -> Hstep'].
+    edestruct fill_redex as [K'' ?]; eauto using head_step_not_val.
+    simplify. rewrite -fill_op in Heq. simplify.
+    exists (K'' @@ e2'). rewrite fill_op; split; first done.
+    apply fill_head_step_val in Hstep as [[v ?] | ?].
+    { apply head_step_not_val in Hstep'. simplify. }
+    simplify. by rewrite !fill_empty.
+  Qed.
+  Lemma head_reducible_prim_step e1 σ1 e2 σ2 :
+    head_reducible e1 σ1 →
+    prim_step e1 σ1 e2 σ2 →
+    head_step e1 σ1 e2 σ2.
+  Proof.
+    intros.
+    edestruct (head_reducible_fill_prim_step ∅) as (? & ? & ?);
+      rewrite ?fill_empty; eauto.
+    by simplify; rewrite fill_empty.
+  Qed.
+
+  Lemma fill_val K e :
+    is_Some (to_val (K @@ e)) →
+    is_Some (to_val e).
+  Proof.
+    rewrite -!not_eq_None_Some. eauto using fill_not_val.
+  Qed.
+  Lemma fill_prim_step_inv K e1' σ1 e2 σ2 :
+    to_val e1' = None →
+    prim_step (K @@ e1') σ1 e2 σ2 →
+    ∃ e2', e2 = K @@ e2' ∧ prim_step e1' σ1 e2' σ2.
+  Proof.
+    intros ? [K_redex e1_redex e2_redex Heq -> Hstep].
+    edestruct fill_redex as [K' ?]; eauto; simplify.
+    rewrite -fill_op in Heq; apply (inj (_ @@.)) in Heq.
+    eexists. rewrite -fill_op. eauto.
+  Qed.
+
+  Global Instance strongly_head_reducible_strongly_reducible e :
+    StronglyHeadReducible e →
+    StronglyReducible e.
+  Proof.
+    intros ? ?. eauto using head_reducible_reducible.
+  Qed.
+  Global Instance strongly_head_irreducible_strongly_irreducible e :
+    StronglyHeadIrreducible e →
+    sub_redexes_are_values e →
+    StronglyIrreducible e.
+  Proof.
+    intros ** ?. eauto using head_irreducible_irreducible.
+  Qed.
+  Global Instance strongly_head_stuck_strongly_stuck e :
+    StronglyHeadStuck e →
+    StronglyStuck e.
+  Proof.
+    intros []. econstructor; last done.
+    eauto using strongly_head_irreducible_strongly_irreducible.
+  Qed.
+
+  Lemma pure_head_step_fill_pure_step K e1 e2 :
+    pure_head_step e1 e2 →
+    pure_step (K @@ e1) (K @@ e2).
+  Proof.
+    intros []. econstructor.
+    - eauto using head_reducible_fill_reducible.
+    - intros * ?%head_reducible_fill_prim_step; naive_solver.
+  Qed.
+  Lemma pure_head_step_pure_step e1 e2 :
+    pure_head_step e1 e2 →
+    pure_step e1 e2.
+  Proof.
+    intros. rewrite -(fill_empty e1) -(fill_empty e2).
+    eauto using pure_head_step_fill_pure_step.
+  Qed.
+  Lemma pure_head_exec_fill_pure_exec K ϕ n e1 e2 :
+    PureHeadExec ϕ n e1 e2 →
+    PureExec ϕ n (K @@ e1) (K @@ e2).
+  Proof.
+    intros ? ?.
+    eapply nsteps_congruence;
+    eauto using pure_head_exec, pure_head_step_fill_pure_step.
+  Qed.
+  Lemma pure_head_exec_pure_exec ϕ n e1 e2 :
+    PureHeadExec ϕ n e1 e2 →
+    PureExec ϕ n e1 e2.
+  Proof.
+    intros. rewrite -(fill_empty e1) -(fill_empty e2).
+    eauto using pure_head_exec_fill_pure_exec.
+  Qed.
+
+  Global Instance fill_lang_frame K :
+    LangFrame (K @@.).
+  Proof.
+    constructor.
+    - apply ectx_lang_mixin.
+    - apply prim_step_fill_prim_step.
+    - apply fill_prim_step_inv.
+  Qed.
+End ectx_lang.
+Global Arguments lang_of_ectx_lang' : clear implicits.
+Coercion lang_of_ectx_lang' : ectx_lang >-> lang.
+
+Definition lang_of_ectx_lang Λ :=
+  let '(@Build_ectx_lang expr val state of_val to_val head_step ectx ectx_base mix) := Λ in
+  @Build_lang expr val state of_val to_val _ $
+  @lang_of_ectx_lang_mixin $
+  Build_ectx_lang mix.
+Global Arguments lang_of_ectx_lang : simpl never.
