theories/without_calls/lang/ectxi_lang.v
@@ -1,0 +1,216 @@
+From simuliris.common Require Import
+  prelude
+  tactics.
+From simuliris.without_calls Require Export
+  lang.ectx_lang.
+
+Section LangEctxiMixin.
+  Context {val expr state : Type}.
+  Context (to_val : expr → option val).
+  Context (head_step : expr → state → expr → state → Prop).
+  Context (ectxi : Type) `{LangCtxiBase expr ectxi}.
+  Implicit Types e : expr.
+  Implicit Types k : ectxi.
+
+  Record LangEctxiMixin := {
+    lang_ectxi_mixin_ctxi_mixin :
+      LangCtxiMixin to_val ectxi ;
+    lang_ectxi_mixin_fill_no_val_inj k1 k2 e1 e2 :
+      to_val e1 = None →
+      to_val e2 = None →
+      k1 @@ e1 = k2 @@ e2 →
+      k1 = k2 ;
+    lang_ectxi_mixin_fill_head_step_val k e1 σ1 e2 σ2 :
+      head_step (k @@ e1) σ1 e2 σ2 →
+      is_Some (to_val e1) ;
+  }.
+End LangEctxiMixin.
+Global Arguments Build_LangEctxiMixin {_ _ _ _ _ _ _} _ _ _ : assert.
+
+Section lang_ectxi_mixin.
+  Context {val expr state : Type}.
+  Context {to_val : expr → option val}.
+  Context {head_step : expr → state → expr → state → Prop}.
+  Context `{LangCtxiBase expr ectxi}.
+  Context (lang_ectxi_mixin : LangEctxiMixin to_val head_step ectxi).
+  Implicit Types k : ectxi.
+
+  Global Instance lang_ectxi_mixin_fill_inj k :
+    Inj (=) (=) (k @@.).
+  Proof.
+    eauto using lang_ectxi_mixin_ctxi_mixin, lang_ctxi_mixin_fill_inj.
+  Qed.
+  Lemma lang_ectxi_mixin_fill_not_val k e :
+    to_val e = None →
+    to_val (k @@ e) = None.
+  Proof.
+    eauto using lang_ectxi_mixin_ctxi_mixin, lang_ctxi_mixin_fill_not_val.
+  Qed.
+  Lemma lang_ectxi_mixin_fill_val k e :
+    is_Some (to_val (k @@ e)) →
+    is_Some (to_val e).
+  Proof.
+    eauto using lang_ectxi_mixin_ctxi_mixin, lang_ctxi_mixin_fill_val.
+  Qed.
+
+  Let ectx := list ectxi.
+  Implicit Types K : ectx.
+
+  Lemma lang_ectxi_mixin_ectx_mixin :
+    ( ∀ e1 σ1 e2 σ2,
+      head_step e1 σ1 e2 σ2 →
+      to_val e1 = None
+    ) →
+    LangEctxMixin to_val head_step ectx.
+  Proof.
+    assert (ectx_fill_op : ∀ K1 K2 e,
+      (K1 ⋅ K2) @@ e = K1 @@ (K2 @@ e)
+    ). {
+      eauto using fold_left_app.
+    }
+    assert (ectx_fill_not_val : ∀ K e,
+      to_val e = None →
+      to_val (K @@ e) = None
+    ). {
+      induction K as [| k K]; intros; first done.
+      naive_solver eauto using IHK, lang_ectxi_mixin_fill_not_val.
+    }
+    assert (ectx_fill_head_step_val : ∀ K e1 σ1 e2 σ2,
+      head_step (K @@ e1) σ1 e2 σ2 →
+      is_Some (to_val e1) ∨ K = ∅
+    ). {
+      induction K as [| k K]; intros * Hstep; first eauto.
+      left. edestruct (IHK (k @@ e1)); first done.
+      + eauto using lang_ectxi_mixin_fill_val.
+      + simplify. cbn in Hstep. eauto using lang_ectxi_mixin_fill_head_step_val.
+    }
+    econstructor.
+    - eauto using lang_ctxi_mixin_ctx_mixin, lang_ectxi_mixin_ctxi_mixin.
+    - intros * Heq ? Hstep. revert K_redex Heq.
+      induction K as [| k K] using rev_ind; intros K_redex Heq.
+      + naive_solver eauto using app_nil_r.
+      + destruct K_redex as [| k_redex K_redex _] using rev_ind; intros.
+        * cbn in Heq. simplify. eapply ectx_fill_head_step_val in Hstep as [].
+          -- exfalso. eapply eq_None_not_Some; eauto.
+          -- exists ∅. done.
+        * rewrite !ectx_fill_op in Heq.
+          assert (k = k_redex) as ->. {
+            eapply lang_ectxi_mixin_fill_no_val_inj; [done | | | done];
+              eapply ectx_fill_not_val; eauto.
+          }
+          simplify. destruct IHK with (K_redex := K_redex) as [K' ->]; eauto.
+          exists K'. setoid_rewrite app_assoc. eauto.
+    - done.
+  Qed.
+End lang_ectxi_mixin.
+
+Section EctxiLangMixin.
+  Context {expr val state : Type}.
+  Context (of_val : val → expr).
+  Context (to_val : expr → option val).
+  Context (head_step : expr → state → expr → state → Prop).
+  Context (ectxi : Type) `{LangCtxiBase expr ectxi}.
+
+  Record EctxiLangMixin := {
+    ectxi_lang_mixin_to_of_val e v :
+      e = of_val v →
+      to_val e = Some v ;
+    ectxi_lang_mixin_of_to_val e v :
+      to_val e = Some v →
+      of_val v = e ;
+    ectxi_lang_mixin_head_step_not_val e1 σ1 e2 σ2 :
+      head_step e1 σ1 e2 σ2 →
+      to_val e1 = None ;
+    ectxi_lang_mixin_ectxi_mixin :
+      LangEctxiMixin to_val head_step ectxi ;
+  }.
+End EctxiLangMixin.
+Global Arguments Build_EctxiLangMixin {_ _ _ _ _ _ _ _} _ _ _ _ : assert.
+
+Structure ectxi_lang := {
+  expr : Type ;
+  val : Type ;
+  state : Type ;
+  of_val : val → expr ;
+  to_val : expr → option val ;
+  head_step : expr → state → expr → state → Prop ;
+  ectxi : Type ;
+  ectxi_lang_ctxi_base : LangCtxiBase expr ectxi ;
+  ectxi_lang_mixin : EctxiLangMixin of_val to_val head_step ectxi ;
+}.
+Global Arguments Build_ectxi_lang {_ _ _ _ _ _ _ _} _ : assert.
+Global Arguments of_val {_} _ : assert.
+Global Arguments to_val {_} _ : assert.
+Global Arguments head_step {_} _ _ _ _ : assert.
+Global Existing Instance ectxi_lang_ctxi_base.
+
+Section ectxi_lang.
+  Context {Λ : ectxi_lang}.
+  Let ectx := list (ectxi Λ).
+  Implicit Types e : expr Λ.
+  Implicit Types k : ectxi Λ.
+  Implicit Types K : ectx.
+
+  Global Instance ectxi_lang_ectx_empty : Empty ectx :=
+    [].
+  Global Instance ectxi_lang_ectx_op : Op ectx :=
+    flip (++).
+  Global Instance ectxi_lang_ectx_fill : Fill ectx (expr Λ) :=
+    fold_left (flip (@@)).
+  Global Instance ectxi_lang_ectx_base : LangCtxBase (expr Λ) ectx :=
+    Build_LangCtxBase _ _ _ _ _.
+
+  Lemma fill_item_not_val k e :
+    to_val e = None →
+    to_val (k @@ e) = None.
+  Proof.
+    apply ectxi_lang_mixin.
+  Qed.
+  Global Instance fill_item_inj k :
+    Inj (=) (=) (k @@.).
+  Proof.
+    apply ectxi_lang_mixin.
+  Qed.
+  Lemma fill_item_no_val_inj k1 k2 e1 e2 :
+    to_val e1 = None →
+    to_val e2 = None →
+    k1 @@ e1 = k2 @@ e2 →
+    k1 = k2.
+  Proof.
+    apply ectxi_lang_mixin.
+  Qed.
+  Lemma fill_item_head_step_val k e σ1 e2 σ2 :
+    head_step (k @@ e) σ1 e2 σ2 →
+    is_Some (to_val e).
+  Proof.
+    apply ectxi_lang_mixin.
+  Qed.
+
+  Lemma fill_item_val k e :
+    is_Some (to_val (k @@ e)) →
+    is_Some (to_val e).
+  Proof.
+    rewrite -!not_eq_None_Some. eauto using fill_item_not_val.
+  Qed.
+
+  Lemma ectx_lang_of_ectxi_lang_mixin :
+    EctxLangMixin of_val to_val head_step ectx.
+  Proof.
+    econstructor;
+      try eapply lang_ectxi_mixin_ectx_mixin;
+      eapply ectxi_lang_mixin.
+  Qed.
+  Canonical ectx_lang_of_ectxi_lang' := Build_ectx_lang ectx_lang_of_ectxi_lang_mixin.
+  Canonical lang_of_ectxi_lang' := lang_of_ectx_lang ectx_lang_of_ectxi_lang'.
+End ectxi_lang.
+Global Arguments ectx_lang_of_ectxi_lang' : clear implicits.
+Global Arguments lang_of_ectxi_lang' : clear implicits.
+Coercion ectx_lang_of_ectxi_lang' : ectxi_lang >-> ectx_lang.
+Coercion lang_of_ectxi_lang' : ectxi_lang >-> lang.
+
+Definition ectx_lang_of_ectxi_lang Λ :=
+  let '(@Build_ectxi_lang expr val state of_val to_val head_step ectxi ectxi_fill mix) := Λ in
+  @Build_ectx_lang expr val state of_val to_val head_step (list ectxi) _ $
+  @ectx_lang_of_ectxi_lang_mixin $
+  Build_ectxi_lang mix.
+Global Arguments ectx_lang_of_ectxi_lang : simpl never.
