theories/without_calls/lang/lang.v
@@ -1,0 +1,412 @@
+From iris.algebra Require Export
+  ofe
+  cmra. (* Op *)
+
+From simuliris.common Require Import
+  prelude
+  tactics.
+From simuliris.common Require Export
+  typeclasses.
+
+Class LangCtxBase expr ctx := {
+  lang_ctx_empty :> Empty ctx ;
+  lang_ctx_op :> Op ctx ;
+  lang_ctx_fill :> Fill ctx expr ;
+}.
+
+Section LangCtxMixin.
+  Context {val expr : Type}.
+  Context (to_val : expr → option val).
+  Context (ctx : Type) `{LangCtxBase expr ctx}.
+  Implicit Types e : expr.
+  Implicit Types C : ctx.
+
+  Record LangCtxMixin := {
+    lang_ctx_mixin_fill_empty e :
+      ∅ @@ e = e ;
+    lang_ctx_mixin_fill_op C1 C2 e :
+      C1 @@ (C2 @@ e) = (C1 ⋅ C2) @@ e ;
+    lang_ctx_mixin_fill_inj C :
+      Inj (=) (=) (C @@.) ;
+    lang_ctx_mixin_fill_not_val C e :
+      to_val e = None →
+      to_val (C @@ e) = None ;
+  }.
+End LangCtxMixin.
+Global Arguments Build_LangCtxMixin {_ _ _ _ _} _ _ _ _ : assert.
+
+Class LangCtxiBase expr ctxi :=
+  lang_ctxi_fill :> Fill ctxi expr.
+
+Section LangCtxiMixin.
+  Context {val expr : Type}.
+  Context (to_val : expr → option val).
+  Context ctxi `{LangCtxiBase expr ctxi}.
+  Implicit Types e : expr .
+  Implicit Types c : ctxi.
+
+  Record LangCtxiMixin := {
+    lang_ctxi_mixin_fill_inj c :
+      Inj (=) (=) (c @@.) ;
+    lang_ctxi_mixin_fill_not_val c e :
+      to_val e = None →
+      to_val (c @@ e) = None ;
+  }.
+End LangCtxiMixin.
+Global Arguments Build_LangCtxiMixin {_ _ _ _ _} _ _ : assert.
+
+Section lang_ctxi_mixin.
+  Context {val expr : Type}.
+  Context {to_val : expr → option val}.
+  Context `{LangCtxiBase expr ctxi}.
+  Context (lang_ctxi_mixin : LangCtxiMixin to_val ctxi).
+
+  Lemma lang_ctxi_mixin_fill_val k e :
+    is_Some (to_val (k @@ e)) →
+    is_Some (to_val e).
+  Proof.
+    rewrite -!not_eq_None_Some. eauto using lang_ctxi_mixin_fill_not_val.
+  Qed.
+
+  Let ctx := list ctxi.
+
+  Global Instance lang_ctxi_mixin_ctx_empty : Empty ctx :=
+    [].
+  Global Instance lang_ctxi_mixin_ctx_op : Op ctx :=
+    flip (++).
+  Global Instance lang_ctxi_mixin_ctx_fill : Fill ctx expr :=
+    fold_left (flip (@@)).
+  Global Instance lang_ctxi_mixin_ctx_base : LangCtxBase expr ctx :=
+    Build_LangCtxBase _ _ _ _ _.
+
+  Lemma lang_ctxi_mixin_ctx_mixin :
+    LangCtxMixin to_val ctx.
+  Proof.
+    econstructor.
+    - done.
+    - simpl. eauto using fold_left_app.
+    - induction C as [| c C]; intros ?**; first eauto.
+      unshelve eapply (inj (c @@.)); eauto using lang_ctxi_mixin_fill_inj.
+    - induction C; naive_solver eauto using lang_ctxi_mixin_fill_not_val.
+  Qed.
+End lang_ctxi_mixin.
+
+Section LangMixin.
+  Context {expr val state : Type}.
+  Context (of_val : val → expr).
+  Context (to_val : expr → option val).
+  Context (prim_step : expr → state → expr → state → Prop).
+
+  Record LangMixin := {
+    lang_mixin_to_of_val e v :
+      e = of_val v →
+      to_val e = Some v ;
+    lang_mixin_of_to_val e v :
+      to_val e = Some v →
+      of_val v = e ;
+    lang_mixin_prim_step_not_val e1 σ1 e2 σ2 :
+      prim_step e1 σ1 e2 σ2 →
+      to_val e1 = None ;
+  }.
+End LangMixin.
+Global Arguments Build_LangMixin {_ _ _ _ _ _} _ _ _ : assert.
+
+Structure lang := {
+  expr : Type ;
+  val : Type ;
+  state : Type ;
+  of_val : val → expr ;
+  to_val : expr → option val ;
+  prim_step : expr → state → expr → state → Prop ;
+  lang_mixin : LangMixin of_val to_val prim_step ;
+}.
+Global Arguments Build_lang {_ _ _ _ _ _} _ : assert.
+Global Arguments of_val {_} _ : assert.
+Global Arguments to_val {_} _ : assert.
+Global Arguments prim_step {_} _ _ _ _ : assert.
+
+Definition cfg Λ := (expr Λ * state Λ)%type.
+
+Canonical Structure stateO Λ := leibnizO (state Λ).
+Canonical Structure valO Λ := leibnizO (val Λ).
+Canonical Structure exprO Λ := leibnizO (expr Λ).
+
+Class LangCtx Λ ctx := {
+  lang_ctx_base :> LangCtxBase (expr Λ) ctx ;
+  lang_ctx_mixin : LangCtxMixin to_val ctx ;
+}.
+Global Arguments Build_LangCtx {_ _ _} _ : assert.
+
+Class LangCtxi Λ ctxi := {
+  lang_ctxi_base :> LangCtxiBase (expr Λ) ctxi ;
+  lang_ctxi_mixin : LangCtxiMixin to_val ctxi ;
+}.
+Global Arguments Build_LangCtxi {_ _ _} _ : assert.
+
+Program Global Instance lang_ctxi_ctx `{LangCtxi Λ ctxi} : LangCtx Λ (list ctxi) :=
+  Build_LangCtx _.
+Next Obligation.
+  eauto using lang_ctxi_mixin_ctx_mixin, lang_ctxi_mixin.
+Qed.
+
+Class LangFrame {Λ : lang} (K : expr Λ → expr Λ) := {
+  lang_frame_not_val e :
+    to_val e = None →
+    to_val (K e) = None ;
+  lang_frame_prim_step e1 σ1 e2 σ2 :
+    prim_step e1 σ1 e2 σ2 →
+    prim_step (K e1) σ1 (K e2) σ2 ;
+  lang_frame_prim_step_inv e1' σ1 e2 σ2 :
+    to_val e1' = None →
+    prim_step (K e1') σ1 e2 σ2 →
+    ∃ e2', e2 = K e2' ∧ prim_step e1' σ1 e2' σ2 ;
+}.
+
+Global Instance lang_frame_id Λ :
+  LangFrame (@id (expr Λ)).
+Proof.
+  constructor; naive_solver.
+Qed.
+
+Section lang.
+  Context {Λ : lang}.
+  Implicit Types v : val Λ.
+  Implicit Types e : expr Λ.
+  Implicit Types σ : state Λ.
+  Implicit Types ρ : cfg Λ.
+
+  Inductive step ρ1 ρ2 : Prop :=
+    | prim_step_step e1 σ1 e2 σ2 :
+        prim_step e1 σ1 e2 σ2 →
+        ρ1 = (e1, σ1) →
+        ρ2 = (e2, σ2) →
+        step ρ1 ρ2.
+  Global Arguments prim_step_step {_ _}.
+  Hint Constructors step : core.
+
+  Definition reducible e σ :=
+    ∃ e' σ', prim_step e σ e' σ'.
+  Definition irreducible e σ :=
+    ∀ e' σ', ¬ prim_step e σ e' σ'.
+  Definition stuck e σ :=
+    irreducible e σ ∧ to_val e = None.
+
+  Class StronglyReducible e :=
+    strongly_reducible σ : reducible e σ.
+  Class StronglyIrreducible e :=
+    strongly_irreducible σ : irreducible e σ.
+  Class StronglyStuck e := {
+    strongly_stuck_strongly_irreducible :> StronglyIrreducible e ;
+    strongly_stuck_not_val : to_val e = None ;
+  }.
+
+  Definition converges e σ e' σ' :=
+    rtc step (e, σ) (e', σ') ∧ irreducible e' σ'.
+
+  CoInductive diverges e σ : Prop :=
+    | diverges_step e' σ' :
+        prim_step e σ e' σ' →
+        diverges e' σ' →
+        diverges e σ.
+
+  Record pure_step e1 e2 := {
+    pure_step_safe σ1 :
+      reducible e1 σ1 ;
+    pure_step_det σ1 e2' σ2 :
+      prim_step e1 σ1 e2' σ2 →
+      σ2 = σ1 ∧ e2' = e2 ;
+  }.
+  Class PureExec (ϕ : Prop) n e1 e2 :=
+    pure_exec : ϕ → nsteps pure_step n e1 e2.
+
+  Lemma to_of_val e v :
+    e = of_val v →
+    to_val e = Some v.
+  Proof.
+    apply lang_mixin.
+  Qed.
+  Lemma of_to_val e v :
+    to_val e = Some v →
+    of_val v = e.
+  Proof.
+    apply lang_mixin.
+  Qed.
+  Lemma prim_step_not_val e1 σ1 e2 σ2 :
+    prim_step e1 σ1 e2 σ2 →
+    to_val e1 = None.
+  Proof.
+    apply lang_mixin.
+  Qed.
+
+  Lemma step_prim_step e1 σ1 e2 σ2 :
+    step (e1, σ1) (e2, σ2) →
+    prim_step e1 σ1 e2 σ2.
+  Proof.
+    intros []. simplify. eauto.
+  Qed.
+  Lemma irreducible_not_reducible e σ :
+    irreducible e σ ↔
+    ¬ reducible e σ.
+  Proof.
+    rewrite /reducible /irreducible. naive_solver.
+  Qed.
+  Lemma reducible_not_val e σ :
+    reducible e σ →
+    to_val e = None.
+  Proof.
+    intros (? & ? & ?); eauto using prim_step_not_val.
+  Qed.
+  Lemma val_irreducible e v σ :
+    e = of_val v →
+    irreducible e σ.
+  Proof.
+    intros ?%to_of_val ? ? ?%prim_step_not_val. naive_solver.
+  Qed.
+  Lemma stuck_irreducible e σ :
+    stuck e σ →
+    irreducible e σ.
+  Proof.
+    rewrite /stuck. naive_solver.
+  Qed.
+  Lemma stuck_not_val e σ :
+    stuck e σ →
+    to_val e = None.
+  Proof.
+    rewrite /stuck. naive_solver.
+  Qed.
+
+  Lemma diverges_reducible e σ :
+    diverges e σ →
+    reducible e σ.
+  Proof.
+    intros []. econstructor. eauto.
+  Qed.
+  Lemma diverges_not_stuck e σ :
+    diverges e σ →
+    ¬ stuck e σ.
+  Proof.
+    by intros ?%diverges_reducible ?%stuck_irreducible%irreducible_not_reducible.
+  Qed.
+  Lemma diverges_not_val e σ v :
+    diverges e σ →
+    e ≠ of_val v.
+  Proof.
+    intros [? ? ? %prim_step_not_val] ?%to_of_val. naive_solver.
+  Qed.
+
+  Lemma strongly_stuck_stuck e σ :
+    StronglyStuck e →
+    stuck e σ.
+  Proof.
+    intros []. econstructor; done.
+  Qed.
+
+  Lemma pure_step_prim_step e1 e2 σ :
+    pure_step e1 e2 →
+    prim_step e1 σ e2 σ.
+  Proof.
+    intros [(? & ? & Hstep) Hdet].
+    specialize (Hdet _ _ _ Hstep). simplify. eauto.
+  Qed.
+  Lemma pure_steps_pure_exec n e1 e2 :
+    nsteps pure_step n e1 e2 →
+    PureExec True n e1 e2.
+  Proof.
+    intros ? ?. done.
+  Qed.
+  Lemma pure_step_pure_exec e1 e2 :
+    pure_step e1 e2 →
+    PureExec True 1 e1 e2.
+  Proof.
+    intros. eapply pure_steps_pure_exec, nsteps_once. done.
+  Qed.
+
+  Lemma rtc_step_val v ρ1 ρ2 :
+    rtc step ρ1 ρ2 →
+    ρ1.1 = of_val v →
+    ρ1 = ρ2.
+  Proof.
+    intros [| [] ? ? [? ? ? ? ?%prim_step_not_val ? ?]] ?%to_of_val;
+      simplify; naive_solver.
+  Qed.
+  Lemma rtc_step_stuck ρ1 ρ2 :
+    rtc step ρ1 ρ2 →
+    stuck ρ1.1 ρ1.2 →
+    ρ1 = ρ2.
+  Proof.
+    intros [| [] ? ? []] Hstuck; simplify; first done.
+    eapply stuck_irreducible in Hstuck. rewrite /irreducible in Hstuck.
+    naive_solver.
+  Qed.
+
+  Section lang_frame.
+    Context (K : expr Λ → expr Λ) `{!LangFrame K}.
+
+    Lemma lang_frame_step e1 σ1 e2 σ2 :
+      step (e1, σ1) (e2, σ2) →
+      step (K e1, σ1) (K e2, σ2).
+    Proof.
+      intros []. simplify.
+      econstructor; auto. eauto using lang_frame_prim_step.
+    Qed.
+    Lemma lang_frame_reducible e σ :
+      reducible e σ →
+      reducible (K e) σ.
+    Proof.
+      rewrite /reducible. naive_solver eauto using lang_frame_prim_step.
+    Qed.
+    Lemma lang_frame_tc_step e1 σ1 e2 σ2 :
+      tc step (e1, σ1) (e2, σ2) →
+      tc step (K e1, σ1) (K e2, σ2).
+    Proof.
+      set K_cfg : cfg Λ → cfg Λ := λ '(e, σ), (K e, σ).
+      change (K ?e, ?σ) with (K_cfg (e, σ)). apply tc_congruence.
+      intros [] []. apply lang_frame_step.
+    Qed.
+    Lemma lang_frame_rtc_step e1 σ1 e2 σ2 :
+      rtc step (e1, σ1) (e2, σ2) →
+      rtc step (K e1, σ1) (K e2, σ2).
+    Proof.
+      intros []%rtc_tc; simplify; eauto using rtc_refl, tc_rtc, lang_frame_tc_step.
+    Qed.
+
+    Lemma lang_frame_reducible_inv e σ :
+      to_val e = None →
+      reducible (K e) σ →
+      reducible e σ.
+    Proof.
+      intros ? (? & ? & (? & -> & ?)%lang_frame_prim_step_inv); last done.
+      rewrite /reducible. eauto.
+    Qed.
+    Lemma lang_frame_irreducible e σ :
+      to_val e = None →
+      irreducible e σ →
+      irreducible (K e) σ.
+    Proof.
+      rewrite !irreducible_not_reducible. eauto using lang_frame_reducible_inv.
+    Qed.
+    Lemma lang_frame_stuck e σ :
+      stuck e σ →
+      stuck (K e) σ.
+    Proof.
+      rewrite /stuck. intros [].
+      split; eauto using lang_frame_not_val, lang_frame_irreducible.
+    Qed.
+
+    Lemma lang_frame_pure_step e1 e2 :
+      pure_step e1 e2 →
+      pure_step (K e1) (K e2).
+    Proof.
+      intros []. econstructor.
+      - eauto using lang_frame_reducible.
+      - intros * Hstep. eapply lang_frame_prim_step_inv in Hstep; first naive_solver.
+        unshelve eauto using reducible_not_val; eauto.
+    Qed.
+    Lemma lang_frame_pure_exec ϕ n e1 e2 :
+      PureExec ϕ n e1 e2 →
+      PureExec ϕ n (K e1) (K e2).
+    Proof.
+      intros ? ?. eapply nsteps_congruence; eauto using lang_frame_pure_step.
+    Qed.
+  End lang_frame.
+End lang.
