theories/without_calls/simul.v
@@ -1,0 +1,692 @@
+From iris.bi Require Import
+  bi
+  fixpoint.
+From iris.base_logic Require Import
+  bi.
+From iris.proofmode Require Import
+  proofmode.
+
+From simuliris.common Require Import
+  prelude
+  tactics.
+From simuliris.common Require Export
+  bi_typeclasses.
+From simuliris.without_calls Require Import
+  lang.ectx_lang
+  refinement.
+
+Class SimulGS (PROP : bi) (Λₜ Λₛ : lang) :=
+  simul_state_interp : state Λₜ → state Λₛ → PROP.
+
+Class Simul (PROP : bi) exprₜ exprₛ :=
+  simul : (exprₜ → exprₛ → PROP) → exprₜ → exprₛ → PROP.
+Local Notation "'SIM' eₜ '≲' eₛ '{{' Φ } }" := (simul Φ eₜ eₛ)
+( at level 70,
+  eₜ, eₛ, Φ at level 200,
+  format "'[hv' 'SIM'  eₜ  ≲  '/   ' eₛ  '/' {{  '[ ' Φ  ']' } } ']'"
+) : bi_scope.
+
+Section bi.
+  Context `{!BiBUpd PROP, !BiAffine PROP, !BiPureForall PROP}.
+  Context `{!BiPlainly PROP, !BiBUpdPlainly PROP}.
+
+  Section lang.
+    Context `{SimulGS PROP Λₜ Λₛ}.
+    Notation expr_rel := (exprO Λₜ -d> exprO Λₛ -d> PROP).
+    Implicit Types eₜ : expr Λₜ.
+    Implicit Types eₛ : expr Λₛ.
+    Implicit Types σₜ : state Λₜ.
+    Implicit Types σₛ : state Λₛ.
+    Implicit Types Φ : expr_rel.
+    Implicit Types Ψ : expr_rel → expr_rel.
+
+    Local Instance expr_rel_func_ne Ψ `{Hne : !NonExpansive Ψ} n :
+      Proper ((≡{n}≡) ==> (≡{n}≡) ==> (≡{n}≡) ==> (≡{n}≡)) Ψ.
+    Proof.
+      intros
+        Φ1 Φ2 HΦ
+        eₜ1 eₜ2 ->%discrete_iff%leibniz_equiv
+        eₛ1 eₛ2 ->%discrete_iff%leibniz_equiv
+      ; [| apply _..].
+      eapply Hne, HΦ.
+    Qed.
+
+    Definition simul_inner (Ψ : expr_rel -d> expr_rel) : expr_rel -d> expr_rel := (
+      λ Φ eₜ eₛ,
+        ∀ σₜ σₛ, simul_state_interp σₜ σₛ ==∗ (
+          simul_state_interp σₜ σₛ ∗ ⌜stuck eₜ σₜ⌝ ∗ ⌜stuck eₛ σₛ⌝
+        ) ∨ (
+          simul_state_interp σₜ σₛ ∗ Φ eₜ eₛ
+        ) ∨ (
+          ∃ eₛ' σₛ', ⌜tc step (eₛ, σₛ) (eₛ', σₛ')⌝ ∗
+          simul_state_interp σₜ σₛ' ∗ Ψ Φ eₜ eₛ'
+        ) ∨ (
+          ⌜reducible eₜ σₜ⌝ ∗ ∀ eₜ' σₜ', ⌜prim_step eₜ σₜ eₜ' σₜ'⌝ ==∗
+          ∃ eₛ' σₛ', ⌜rtc step (eₛ, σₛ) (eₛ', σₛ')⌝ ∗
+          simul_state_interp σₜ' σₛ' ∗ Ψ Φ eₜ' eₛ'
+        )
+    )%I.
+
+    Instance simul_inner_ne n :
+      Proper (
+        ((≡{n}≡) ==> (≡{n}≡) ==> (≡{n}≡)) ==>
+        ((≡{n}≡) ==> (≡{n}≡) ==> (≡{n}≡)) ==>
+        (≡{n}≡) ==> (≡{n}≡) ==> (≡{n}≡)
+      ) simul_inner.
+    Proof.
+      intros
+        Ψ1 Ψ2 HΨ Φ1 Φ2 HΦ
+        eₜ1 eₜ2 Heₜ%discrete_iff%leibniz_equiv
+        eₛ1 eₛ2 Heₛ%discrete_iff%leibniz_equiv
+      ; [| apply _..].
+      subst. rewrite /simul_inner.
+      repeat (f_equiv || apply HΦ || eapply HΨ || reflexivity || intros ? ?).
+    Qed.
+    Instance simul_inner_proper :
+      Proper (
+        ((≡) ==> (≡) ==> (≡)) ==>
+        ((≡) ==> (≡) ==> (≡)) ==>
+        (≡) ==> (≡) ==> (≡)
+      ) simul_inner.
+    Proof.
+      intros
+        Ψ1 Ψ2 HΨ Φ1 Φ2 HΦ
+        eₜ1 eₜ2 Heₜ%leibniz_equiv
+        eₛ1 eₛ2 Heₛ%leibniz_equiv.
+      subst. rewrite /simul_inner.
+      repeat (f_equiv || apply HΦ || eapply HΨ || reflexivity || intros ? ?).
+    Qed.
+
+    Lemma simul_inner_mono Ψ1 Ψ2 :
+      ⊢ □ (Ψ1 --∗ Ψ2) →
+        simul_inner Ψ1 --∗ simul_inner Ψ2.
+    Proof.
+      iIntros "#Hmono" (? ? ?) " Hsimul". rewrite /simul_inner. iIntros "* Hinv".
+      iMod ("Hsimul" with "Hinv") as "[? | [? | [Hsimul | Hsimul]]]"; iModIntro.
+      - eauto.
+      - eauto.
+      - do 2 iRight. iLeft.
+        iDestruct "Hsimul" as (? ?) "(% & ? & ?)".
+        repeat iExists _. iFrame. iSplit; first done.
+        iApply ("Hmono" with "[$]").
+      - do 3 iRight.
+        iDestruct "Hsimul" as "($ & Hsimul)".
+        iIntros "* %".
+        iMod ("Hsimul" with "[//]") as (? ?) "(% & ? & ?)". iModIntro.
+        repeat iExists _. iFrame. iSplit; first done.
+        by iApply "Hmono".
+    Qed.
+    Lemma simul_inner_strong_mono Ψ1 Ψ2 :
+      ⊢ □ (∀ Φ1 Φ2, (Φ1 ===∗ Φ2) -∗ Ψ1 Φ1 --∗ Ψ2 Φ2) →
+        ∀ Φ1 Φ2, (Φ1 ===∗ Φ2) -∗ simul_inner Ψ1 Φ1 --∗ simul_inner Ψ2 Φ2.
+    Proof.
+      iIntros "#Hmono * HΦ" (? ?) "Hsimul". rewrite /simul_inner. iIntros "* Hinv".
+      iMod ("Hsimul" with "Hinv") as "[Hsimul | [Hsimul | [Hsimul | Hsimul]]]".
+      - eauto.
+      - iDestruct "Hsimul" as "(? & ?)".
+        iMod ("HΦ" with "[$]"). iModIntro.
+        iRight. iLeft. iFrame.
+      - iModIntro. do 2 iRight. iLeft.
+        iDestruct "Hsimul" as (? ?) "(% & ? & ?)".
+        repeat iExists _. iFrame. iSplit; first eauto.
+        iApply ("Hmono" with "[$] [$]").
+      - iModIntro. do 3 iRight.
+        iDestruct "Hsimul" as "($ & Hsimul)".
+        iIntros "* %".
+        iMod ("Hsimul" with "[//]") as (? ? ?) "(? & ?)". iModIntro.
+        repeat iExists _. iFrame. iSplit; first eauto.
+        iApply ("Hmono" with "[$] [$]").
+    Qed.
+
+    Definition simul_body (Ψ : prodO (prodO expr_rel (exprO Λₜ)) (exprO Λₛ) → PROP)
+    : prodO (prodO expr_rel (exprO Λₜ)) (exprO Λₛ) → PROP :=
+      uncurry3 $ simul_inner $ curry3 Ψ.
+    Local Instance :
+      BiMonoPred simul_body.
+    Proof.
+      constructor.
+      - iIntros (Φ1 Φ2 HΦ1 HΦ2) "#HΦ". iIntros ([[Φ eₜ] eₛ]). simpl.
+        iApply (simul_inner_mono with "[]"); iModIntro.
+        iIntros (? ? ?). iApply "HΦ".
+      - intros Ψ HΨ n [[Φ1 eₜ1] eₛ1] [[Φ2 eₜ2] eₛ2] [[HΦ]].
+        eapply simul_inner_ne; eauto.
+        + intros ? ? ? ? ? ? ?. eapply HΨ. done.
+        + intros ? ? ->%leibniz_equiv ? ? ->%leibniz_equiv. eapply HΦ.
+    Qed.
+    Global Instance simul_bi_simul : Simul PROP (expr Λₜ) (expr Λₛ) :=
+      curry3 $ bi_least_fixpoint simul_body.
+
+    Lemma simul_eq :
+      simul = curry3 $ bi_least_fixpoint simul_body.
+    Proof.
+      done.
+    Qed.
+    Lemma simul_fixpoint eₜ eₛ Φ :
+      SIM eₜ ≲ eₛ {{ Φ }}%I ≡ simul_inner simul Φ eₜ eₛ.
+    Proof.
+      rewrite simul_eq /curry3 least_fixpoint_unfold /uncurry3 //=.
+    Qed.
+    Lemma simul_unfold eₜ eₛ Φ :
+      SIM eₜ ≲ eₛ {{ Φ }}%I ≡
+      ( ∀ σₜ σₛ, simul_state_interp σₜ σₛ ==∗ (
+          simul_state_interp σₜ σₛ ∗ ⌜stuck eₜ σₜ⌝ ∗ ⌜stuck eₛ σₛ⌝
+        ) ∨ (
+          simul_state_interp σₜ σₛ ∗ Φ eₜ eₛ
+        ) ∨ (
+          ∃ eₛ' σₛ', ⌜tc step (eₛ, σₛ) (eₛ', σₛ')⌝ ∗
+          simul_state_interp σₜ σₛ' ∗ SIM eₜ ≲ eₛ' {{ Φ }}
+        ) ∨ (
+          ⌜reducible eₜ σₜ⌝ ∗ ∀ eₜ' σₜ', ⌜prim_step eₜ σₜ eₜ' σₜ'⌝ ==∗
+          ∃ eₛ' σₛ', ⌜rtc step (eₛ, σₛ) (eₛ', σₛ')⌝ ∗
+          simul_state_interp σₜ' σₛ' ∗ SIM eₜ' ≲ eₛ' {{ Φ }}
+        )
+      )%I.
+    Proof.
+      by rewrite simul_fixpoint.
+    Qed.
+
+    Lemma simul_strong_ind Ψ :
+      NonExpansive Ψ →
+      ⊢ □ (simul_inner (Ψ ⊓ simul) --∗ Ψ) -∗
+        simul --∗ Ψ.
+    Proof.
+      iIntros (?) "#Hind". iIntros (Φ eₜ eₛ) "?".
+      change (Ψ Φ eₜ eₛ) with (uncurry3 Ψ (Φ, eₜ, eₛ)).
+      iApply (least_fixpoint_ind with "[#] [$]").
+      iIntros "!>" ([[]]) "**".
+      iApply ("Hind" with "[$]").
+    Qed.
+    Lemma simul_ind Ψ :
+      NonExpansive Ψ →
+      ⊢ □ (simul_inner Ψ --∗ Ψ) -∗
+        simul --∗ Ψ.
+    Proof.
+      iIntros (?) "#Hind". iIntros (? ? ?) "?".
+      iApply simul_strong_ind; last done.
+      iIntros "!>" (? ? ?) "?".
+      iApply "Hind". iApply simul_inner_mono; last done.
+      iIntros "!>" (? ? ?) "H". iEval (cbv) in "H". by iDestruct "H" as "(? & _)".
+    Qed.
+
+    Lemma simul_bupd_mono Φ1 Φ2 :
+      (Φ1 ===∗ Φ2) -∗
+      simul Φ1 --∗ simul Φ2.
+    Proof.
+      iIntros "**" (eₜ eₛ) "**".
+      iApply (simul_strong_ind (
+        λ Φ1 eₜ eₛ,
+          ∀ Φ2, (Φ1 ===∗ Φ2) -∗ SIM eₜ ≲ eₛ {{ Φ2 }}
+      )%I with "[#] [$]"); [solve_proper | | done].
+      iIntros "!>". clear eₜ eₛ. iIntros (Φ eₜ eₛ) "Hsimul **".
+      iEval (rewrite simul_fixpoint).
+      iApply (simul_inner_strong_mono with "[#] [$]"); last done.
+      iIntros "!> **" (? ?) "Hind".
+      by iApply "Hind".
+    Qed.
+    Lemma simul_mono Φ1 Φ2 :
+      (Φ1 --∗ Φ2) -∗
+      simul Φ1 --∗ simul Φ2.
+    Proof.
+      iIntros "HΦ" (? ?) "**".
+      iApply (simul_bupd_mono with "[HΦ] [$]").
+      by iApply bi_pred2_wand_wand_bupd.
+    Qed.
+
+    Lemma simul_bupd Φ :
+      ⊢ simul (|==> Φ) --∗ simul Φ.
+    Proof.
+      iApply simul_bupd_mono. by iIntros (? ?) "?".
+    Qed.
+    Lemma bupd_simul :
+      ⊢ (|==> simul) --∗ simul.
+    Proof.
+      iIntros (? ? ?) "Hsimul". iApply simul_unfold. iIntros.
+      iMod "Hsimul". rewrite simul_fixpoint. by iMod ("Hsimul" with "[$]").
+    Qed.
+
+    Lemma simul_frame_r R eₜ eₛ Φ :
+      SIM eₜ ≲ eₛ {{ Φ }} ∗ R -∗
+      SIM eₜ ≲ eₛ {{ λ eₜ' eₛ', Φ eₜ' eₛ' ∗ R }}.
+    Proof.
+      iIntros "(? & HR)".
+      iApply (simul_mono with "[HR] [$]").
+      iIntros (? ?) "?". iSplitR "HR"; eauto.
+    Qed.
+    Lemma simul_frame_l R eₜ eₛ Φ :
+      R ∗ SIM eₜ ≲ eₛ {{ Φ }} -∗
+      SIM eₜ ≲ eₛ {{ λ eₜ' eₛ', R ∗ Φ eₜ' eₛ' }}.
+    Proof.
+      iIntros "(HR & ?)".
+      iApply (simul_mono with "[HR] [$]").
+      iIntros (? ?) "?". iSplitL "HR"; eauto.
+    Qed.
+
+    Lemma simul_update_state_interp eₜ eₛ Φ :
+      ( ∀ σₜ σₛ,
+        simul_state_interp σₜ σₛ ==∗
+        simul_state_interp σₜ σₛ ∗ SIM eₜ ≲ eₛ {{ Φ }}
+      ) -∗
+      SIM eₜ ≲ eₛ {{ Φ }}.
+    Proof.
+      iIntros "H". iApply simul_unfold. iIntros.
+      iMod ("H" with "[$]") as "(? & H)".
+      iEval (rewrite simul_unfold) in "H". iApply ("H" with "[$]").
+    Qed.
+
+    Lemma simul_stuck eₜ eₛ Φ :
+      ( ∀ σₜ σₛ,
+        simul_state_interp σₜ σₛ -∗
+        simul_state_interp σₜ σₛ ∗ ⌜stuck eₜ σₜ ∧ stuck eₛ σₛ⌝
+      ) -∗
+      SIM eₜ ≲ eₛ {{ Φ }}.
+    Proof.
+      iIntros "H". iApply simul_unfold. iIntros. iLeft. iModIntro.
+      iDestruct ("H" with "[$]") as "(? & % & %)". eauto.
+    Qed.
+    Lemma simul_strongly_stuck eₜ eₛ Φ :
+      StronglyStuck eₜ →
+      StronglyStuck eₛ →
+      ⊢ SIM eₜ ≲ eₛ {{ Φ }}.
+    Proof.
+      iIntros. iApply simul_stuck. iIntros. iFrame.
+      eauto using strongly_stuck_stuck.
+    Qed.
+
+    Lemma simul_post Φ :
+      ⊢ Φ --∗ simul Φ.
+    Proof.
+      iIntros (? ?) "?". iApply simul_unfold. iIntros. iModIntro.
+      iRight. iLeft. iFrame.
+    Qed.
+
+    Lemma simul_bind Kₜ `{!LangFrame Kₜ} Kₛ `{!LangFrame Kₛ} eₜ eₛ Φ :
+      SIM eₜ ≲ eₛ {{ λ eₜ' eₛ', SIM Kₜ eₜ' ≲ Kₛ eₛ' {{ Φ }} }} -∗
+      SIM Kₜ eₜ ≲ Kₛ eₛ {{ Φ }}.
+    Proof.
+      set Ψ : expr_rel → expr_rel := (
+        λ Φ' eₜ' eₛ',
+          (∀ eₜ'' eₛ'', Φ' eₜ'' eₛ'' -∗ SIM Kₜ eₜ'' ≲ Kₛ eₛ'' {{ Φ }}) -∗
+          SIM Kₜ eₜ' ≲ Kₛ eₛ' {{ Φ }}
+      )%I.
+      cut (⊢ simul --∗ Ψ).
+      { iIntros (HΨ) "**". iApply (HΨ with "[$]"). eauto. }
+      clear eₜ eₛ. iApply simul_ind; first solve_proper.
+      iIntros "!>" (Φ' eₜ' eₛ') "Hsimul Hcont".
+      iApply simul_unfold. iIntros "**".
+      iMod ("Hsimul" with "[$]") as "[Hsimul | [Hsimul | [Hsimul | Hsimul]]]".
+      - iDestruct "Hsimul" as "(? & % & %)".
+        iModIntro. iLeft. iFrame. iSplit; iPureIntro; eauto using lang_frame_stuck.
+      - iDestruct "Hsimul" as "(? & ?)".
+        iDestruct (simul_fixpoint with "(Hcont [$])") as "Hsimul".
+        iMod ("Hsimul" with "[$]"). iModIntro. iFrame.
+      - iDestruct "Hsimul" as (? ?) "(% & ? & Hsimul)".
+        iModIntro. do 2 iRight. iLeft. repeat iExists _. iSplit.
+        + iPureIntro. apply lang_frame_tc_step; done.
+        + iFrame. iApply "Hsimul". iFrame.
+      - iDestruct "Hsimul" as "(% & Hsimul)".
+        iModIntro. do 3 iRight. iSplit.
+        + iPureIntro. eapply lang_frame_reducible; eauto.
+        + iIntros "* %Hstep".
+          apply lang_frame_prim_step_inv in Hstep as (? & -> & ?); first last.
+          { eauto using reducible_not_val. }
+          iMod ("Hsimul" with "[%]") as (? ?) "(% & ? & HΨ)"; first done.
+          iModIntro. repeat iExists _. iSplit.
+          * iPureIntro. apply lang_frame_rtc_step; eauto.
+          * iFrame. by iApply "HΨ".
+    Qed.
+    Lemma simul_decompose Φ1 Φ2 :
+      (Φ1 --∗ simul Φ2) -∗
+      simul Φ1 --∗ simul Φ2.
+    Proof.
+      iIntros "HΦ" (eₜ eₛ) "?".
+      iEval (change eₜ with (id eₜ); change eₛ with (id eₛ)).
+      iApply simul_bind. iApply (simul_mono with "[HΦ //] [$]").
+    Qed.
+
+    Lemma simul_steps eₜ eₛ Φ :
+      ( ∀ σₜ σₛ, simul_state_interp σₜ σₛ ==∗
+        ⌜reducible eₜ σₜ⌝ ∗ ∀ eₜ' σₜ', ⌜prim_step eₜ σₜ eₜ' σₜ'⌝ ==∗
+        ∃ eₛ' σₛ', ⌜rtc step (eₛ, σₛ) (eₛ', σₛ')⌝ ∗
+        simul_state_interp σₜ' σₛ' ∗ SIM eₜ' ≲ eₛ' {{ Φ }}
+      ) -∗
+      SIM eₜ ≲ eₛ {{ Φ }}.
+    Proof.
+      iIntros "H". iApply simul_unfold. iIntros.
+      iMod ("H" with "[$]") as "(% & H)". iModIntro.
+      do 3 iRight. iSplit; first done. iIntros.
+      iMod ("H" with "[//]") as (? ?) "(% & ? & ?)". iModIntro.
+      repeat iExists _. iFrame. done.
+    Qed.
+    Lemma simul_step eₜ eₛ Φ :
+      ( ∀ σₜ σₛ, simul_state_interp σₜ σₛ ==∗
+        ⌜reducible eₜ σₜ⌝ ∗ ∀ eₜ' σₜ', ⌜prim_step eₜ σₜ eₜ' σₜ'⌝ ==∗
+        ∃ eₛ' σₛ', ⌜prim_step eₛ σₛ eₛ' σₛ'⌝ ∗
+        simul_state_interp σₜ' σₛ' ∗ SIM eₜ' ≲ eₛ' {{ Φ }}
+      ) -∗
+      SIM eₜ ≲ eₛ {{ Φ }}.
+    Proof.
+      iIntros "H". iApply simul_steps.
+      iIntros. iMod ("H" with "[$]") as "($ & H)". iModIntro.
+      iIntros. iMod ("H" with "[//]") as (? ?) "(% & ? & ?)". iModIntro.
+      repeat iExists _. iFrame. eauto using rtc_once, prim_step_step.
+    Qed.
+
+    Lemma simul_stepₜ eₜ eₛ Φ :
+      ( ∀ σₜ σₛ, simul_state_interp σₜ σₛ ==∗
+        ⌜reducible eₜ σₜ⌝ ∗ ∀ eₜ' σₜ', ⌜prim_step eₜ σₜ eₜ' σₜ'⌝ ==∗
+        simul_state_interp σₜ' σₛ ∗ SIM eₜ' ≲ eₛ {{ Φ }}
+      ) -∗
+      SIM eₜ ≲ eₛ {{ Φ }}.
+    Proof.
+      iIntros "H". iApply simul_steps. iIntros.
+      iMod ("H" with "[$]") as "(% & H)". iModIntro.
+      iSplit; first done. iIntros.
+      iMod ("H" with "[//]") as "(? & ?)". iModIntro.
+      repeat iExists _. iFrame. done.
+    Qed.
+    Lemma simul_stepsₛ eₜ eₛ Φ :
+      ( ∀ σₜ σₛ, simul_state_interp σₜ σₛ ==∗
+        ∃ eₛ' σₛ', ⌜rtc step (eₛ, σₛ) (eₛ', σₛ')⌝ ∗
+        simul_state_interp σₜ σₛ' ∗ SIM eₜ ≲ eₛ' {{ Φ }}
+      ) -∗
+      SIM eₜ ≲ eₛ {{ Φ }}.
+    Proof.
+      iIntros "H". iApply simul_unfold. iIntros.
+      iMod ("H" with "[$]") as (? ? []%rtc_tc) "(? & Hsim)".
+      - simplify. iEval (rewrite simul_unfold) in "Hsim".
+        iMod ("Hsim" with "[$]"). iModIntro. done.
+      - iModIntro. do 2 iRight. iLeft. repeat iExists _. iFrame. done.
+    Qed.
+    Lemma simul_stepₛ eₜ eₛ Φ :
+      ( ∀ σₜ σₛ, simul_state_interp σₜ σₛ ==∗
+        ∃ eₛ' σₛ', ⌜prim_step eₛ σₛ eₛ' σₛ'⌝ ∗
+        simul_state_interp σₜ σₛ' ∗ SIM eₜ ≲ eₛ' {{ Φ }}
+      ) -∗
+      SIM eₜ ≲ eₛ {{ Φ }}.
+    Proof.
+      iIntros "H". iApply simul_stepsₛ. iIntros.
+      iMod ("H" with "[$]") as (? ?) "(% & ? & ?)". iModIntro.
+      repeat iExists _. iFrame. eauto using rtc_once, prim_step_step.
+    Qed.
+
+    Lemma simul_pure_stepₜ eₜ1 eₜ2 eₛ Φ :
+      pure_step eₜ1 eₜ2 →
+      SIM eₜ2 ≲ eₛ {{ Φ }} -∗
+      SIM eₜ1 ≲ eₛ {{ Φ }}.
+    Proof.
+      iIntros ([]) "**". iApply simul_stepₜ. iIntros. iModIntro.
+      iSplit; first done. iIntros "*" (?%pure_step_det) "!>". simplify. iFrame.
+    Qed.
+    Lemma simul_pure_execₜ ϕ n eₜ1 eₜ2 eₛ Φ :
+      PureExec ϕ n eₜ1 eₜ2 →
+      ϕ →
+      SIM eₜ2 ≲ eₛ {{ Φ }} -∗
+      SIM eₜ1 ≲ eₛ {{ Φ }}.
+    Proof.
+      intros * HPureExec Hsteps%pure_exec.
+      generalize eₜ1 Hsteps. clear HPureExec Hsteps.
+      induction n; intros * Hsteps; invert Hsteps; first done.
+      iIntros. iApply simul_pure_stepₜ; first done. iApply IHn; eauto.
+    Qed.
+
+    Lemma simul_pure_execₛ ϕ n eₜ eₛ1 eₛ2 Φ :
+      PureExec ϕ n eₛ1 eₛ2 →
+      ϕ →
+      SIM eₜ ≲ eₛ2 {{ Φ }} -∗
+      SIM eₜ ≲ eₛ1 {{ Φ }}.
+    Proof.
+      iIntros (? ?%pure_exec%rtc_nsteps_2) "**".
+      iApply simul_stepsₛ. iIntros. iModIntro.
+      repeat iExists _. iFrame. iPureIntro.
+      eapply rtc_congruence with (f := (., _)); last done.
+      eauto using prim_step_step, pure_step_prim_step.
+    Qed.
+    Lemma simul_pure_stepₛ eₜ eₛ1 eₛ2 Φ :
+      pure_step eₛ1 eₛ2 →
+      SIM eₜ ≲ eₛ2 {{ Φ }} -∗
+      SIM eₜ ≲ eₛ1 {{ Φ }}.
+    Proof.
+      iIntros. iApply simul_pure_execₛ; eauto using pure_step_pure_exec.
+    Qed.
+
+    Section adequacy.
+      Context `{Similar (val Λₜ) (val Λₛ)}.
+      Context `{BiSimilar PROP (val Λₜ) (val Λₛ)}.
+      Context (val_equiv_adequacy : ∀ vₜ vₛ, vₜ ≈ vₛ -∗ ⌜vₜ ≈ vₛ⌝).
+
+      Definition simul_post_val eₜ eₛ := (
+        ∃ vₜ vₛ, ⌜eₜ = of_val vₜ⌝ ∗ ⌜eₛ = of_val vₛ⌝ ∗ vₜ ≈ vₛ
+      )%I.
+
+      Lemma simul_converges eₜ σₜ eₜ' σₜ' eₛ σₛ :
+        SIM eₜ ≲ eₛ {{ simul_post_val }} -∗
+        simul_state_interp σₜ σₛ -∗
+        ⌜converges eₜ σₜ eₜ' σₜ'⌝ -∗
+        ⌜ ∃ eₛ' σₛ',
+          converges eₛ σₛ eₛ' σₛ' ∧
+          behaviour_converges eₜ' ⊴ behaviour_converges eₛ'
+        ⌝.
+      Proof.
+        set Ψ : expr_rel → expr_rel := (
+          λ Φ eₜ eₛ,
+            ∀ σₜ σₛ eₜ' σₜ',
+            (Φ --∗ simul_post_val) -∗
+            simul_state_interp σₜ σₛ -∗
+            ⌜converges eₜ σₜ eₜ' σₜ'⌝ -∗
+            ⌜ ∃ eₛ' σₛ',
+              converges eₛ σₛ eₛ' σₛ' ∧
+              behaviour_converges eₜ' ⊴ behaviour_converges eₛ'
+            ⌝
+        )%I.
+        cut (⊢ simul --∗ Ψ).
+        { iIntros (HΨ) "**". iApply (HΨ with "[$] [] [$] [//]").
+          by iIntros (? ?) "**".
+        }
+        clear eₜ σₜ eₜ' σₜ' eₛ σₛ. iApply simul_ind; first solve_proper.
+        iIntros "!>" (Φ eₜ eₛ) "Hsimul". iIntros (σₜ σₛ eₜ' σₜ') "HΦ ? (%Hsteps & %)".
+        iMod ("Hsimul" with "[$]") as "[Hsimul | [Hsimul | [Hsimul | Hsimul]]]".
+        - iDestruct "Hsimul" as "(? & % & %)".
+          iPureIntro. repeat eexists.
+          + eauto using rtc_refl.
+          + eauto using stuck_irreducible.
+          + eapply rtc_step_stuck in Hsteps; last done. simplify.
+            eapply behaviour_refinement_stuck; eauto using stuck_not_val.
+        - iDestruct "Hsimul" as "(_ & ?)".
+          iDestruct ("HΦ" with "[$]") as "(% & % & % & % & ?)".
+          iDestruct (val_equiv_adequacy with "[$]") as "%".
+          iPureIntro. exists eₛ, σₛ. split; first split.
+          * eauto using rtc_refl.
+          * eauto using val_irreducible.
+          * eapply rtc_step_val in Hsteps; last done. simplify.
+            eapply behaviour_refinement_val; eauto.
+        - iDestruct "Hsimul" as (? ?) "(% & ? & HΨ)".
+          iDestruct ("HΨ" with "[$] [$] [//]") as "%Hconv".
+          rewrite /converges in Hconv. simplify.
+          iPureIntro. repeat eexists; eauto. eauto using tc_rtc, tc_rtc_r.
+        - iDestruct "Hsimul" as "(% & Hsimul)".
+          inversion Hsteps as [| ? []]; simplify; first firstorder.
+          iMod ("Hsimul" with "[%]") as (? ? ?) "(? & HΨ)".
+          { eauto using step_prim_step. }
+          iDestruct ("HΨ" with "[$] [$] [//]") as "%Hconv".
+          rewrite /converges in Hconv. simplify.
+          iPureIntro. repeat eexists; [by etrans | eauto..].
+      Qed.
+      Lemma simul_diverges eₜ σₜ eₛ σₛ :
+        SIM eₜ ≲ eₛ {{ simul_post_val }} -∗
+        simul_state_interp σₜ σₛ -∗
+        ⌜diverges eₜ σₜ⌝ -∗
+        False.
+      Proof.
+        set Ψ : expr_rel → expr_rel := (
+          λ Φ eₜ _,
+            ∀ σₜ σₛ,
+            (Φ --∗ simul_post_val) -∗
+            simul_state_interp σₜ σₛ -∗
+            ⌜diverges eₜ σₜ⌝ -∗
+            False
+        )%I.
+        cut (⊢ simul --∗ Ψ).
+        { iIntros (HΨ) "**". iApply (HΨ with "[$] [] [$] [//]").
+          by iIntros (? ?) "**".
+        }
+        clear eₜ σₜ eₛ σₛ. iApply simul_ind; first solve_proper.
+        iIntros "!>" (Φ eₜ eₛ) "Hsimul". iIntros (? ?) "HΦ ? %Hdiv".
+        iMod ("Hsimul" with "[$]") as "[Hsimul | [Hsimul | [Hsimul | Hsimul]]]".
+        - iDestruct "Hsimul" as "(? & % & %)".
+          iPureIntro. eapply diverges_not_stuck; eauto.
+        - iDestruct "Hsimul" as "(_ & Hsimul)".
+          iDestruct ("HΦ" with "[$]") as "(% & % & % & _)".
+          iPureIntro. eapply diverges_not_val; eauto.
+        - iDestruct "Hsimul" as (? ?) "(% & ? & Hsimul)".
+          iApply ("Hsimul" with "[$] [$] [//]").
+        - iDestruct "Hsimul" as "(_ & Hsimul)". destruct Hdiv.
+          iMod ("Hsimul" with "[%]") as (? ?) "(% & ? & HΨ)"; first done.
+          iApply ("HΨ" with "[$] [$] [//]").
+      Qed.
+      Lemma simul_refinement eₜ σₜ eₛ σₛ :
+        SIM eₜ ≲ eₛ {{ simul_post_val }} -∗
+        simul_state_interp σₜ σₛ -∗
+        ⌜(eₜ, σₜ) ⊴ (eₛ, σₛ)⌝.
+      Proof.
+        iIntros "? ?" (? []).
+        - iDestruct (simul_converges with "[$] [$] [//]") as "%". simplify.
+          iPureIntro. eexists. split; last eauto. econstructor. eauto.
+        - iDestruct (simul_diverges with "[$] [$] [//]") as "[]".
+      Qed.
+    End adequacy.
+  End lang.
+
+  Section ectx_lang.
+    Context {Λₜ : ectx_lang} {Λₛ : ectx_lang}.
+    Context `{SimulGS PROP Λₜ Λₛ}.
+    Implicit Types eₜ : expr Λₜ.
+    Implicit Types eₛ : expr Λₛ.
+    Implicit Types σₜ : state Λₜ.
+    Implicit Types σₛ : state Λₛ.
+    Implicit Types Kₜ : ectx Λₜ.
+    Implicit Types Kₛ : ectx Λₛ.
+
+    Lemma simul_bind' Kₜ Kₛ eₜ eₛ Φ :
+      SIM eₜ ≲ eₛ {{ λ eₜ' eₛ', SIM Kₜ @@ eₜ' ≲ Kₛ @@ eₛ' {{ Φ }} }} -∗
+      SIM Kₜ @@ eₜ ≲ Kₛ @@ eₛ {{ Φ }}.
+    Proof.
+      rewrite simul_bind //.
+    Qed.
+
+    Lemma simul_head_step eₜ eₛ Φ :
+      ( ∀ σₜ σₛ, simul_state_interp σₜ σₛ ==∗
+        ⌜head_reducible eₜ σₜ⌝ ∗ ∀ eₜ' σₜ', ⌜head_step eₜ σₜ eₜ' σₜ'⌝ ==∗
+        ∃ eₛ' σₛ', ⌜head_step eₛ σₛ eₛ' σₛ'⌝ ∗
+        simul_state_interp σₜ' σₛ' ∗ SIM eₜ' ≲ eₛ' {{ Φ }}
+      ) -∗
+      SIM eₜ ≲ eₛ {{ Φ }}.
+    Proof.
+      iIntros "H". iApply simul_step.
+      iIntros. iMod ("H" with "[$]") as "(% & H)". iModIntro.
+      iSplit; first eauto using head_reducible_reducible.
+      iIntros "*" (?%head_reducible_prim_step); last done.
+      iMod ("H" with "[//]") as (? ?) "(% & ? & ?)". iModIntro.
+      repeat iExists _. iSplit; last iFrame.
+      naive_solver eauto using head_step_prim_step.
+    Qed.
+
+    Lemma simul_head_stepₜ eₜ eₛ Φ :
+      ( ∀ σₜ σₛ, simul_state_interp σₜ σₛ ==∗
+        ⌜head_reducible eₜ σₜ⌝ ∗ ∀ eₜ' σₜ', ⌜head_step eₜ σₜ eₜ' σₜ'⌝ ==∗
+        simul_state_interp σₜ' σₛ ∗ SIM eₜ' ≲ eₛ {{ Φ }}
+      ) -∗
+      SIM eₜ ≲ eₛ {{ Φ }}.
+    Proof.
+      iIntros "H". iApply simul_stepₜ. iIntros.
+      iMod ("H" with "[$]") as "(% & H)". iModIntro.
+      iSplit; first eauto using head_reducible_reducible.
+      iIntros "*" (?%head_reducible_prim_step); last done.
+      iMod ("H" with "[//]") as "(? & ?)". iModIntro. iFrame.
+    Qed.
+    Lemma simul_head_stepₛ eₜ eₛ Φ :
+      ( ∀ σₜ σₛ, simul_state_interp σₜ σₛ ==∗
+        ∃ eₛ' σₛ', ⌜head_step eₛ σₛ eₛ' σₛ'⌝ ∗
+        simul_state_interp σₜ σₛ' ∗ SIM eₜ ≲ eₛ' {{ Φ }}
+      ) -∗
+      SIM eₜ ≲ eₛ {{ Φ }}.
+    Proof.
+      iIntros "H". iApply simul_stepₛ. iIntros.
+      iMod ("H" with "[$]") as (? ?) "(% & ? & ?)". iModIntro.
+      repeat iExists _. iFrame. iPureIntro. by eapply head_step_prim_step.
+    Qed.
+
+    Lemma simul_pure_head_stepₜ eₜ1 eₜ2 eₛ Φ :
+      pure_head_step eₜ1 eₜ2 →
+      SIM eₜ2 ≲ eₛ {{ Φ }} -∗
+      SIM eₜ1 ≲ eₛ {{ Φ }}.
+    Proof.
+      iIntros. iApply simul_pure_stepₜ; eauto using pure_head_step_pure_step.
+    Qed.
+    Lemma simul_pure_head_execₜ ϕ n eₜ1 eₜ2 eₛ Φ :
+      PureHeadExec ϕ n eₜ1 eₜ2 →
+      ϕ →
+      SIM eₜ2 ≲ eₛ {{ Φ }} -∗
+      SIM eₜ1 ≲ eₛ {{ Φ }}.
+    Proof.
+      iIntros. iApply simul_pure_execₜ; eauto using pure_head_exec_pure_exec.
+    Qed.
+
+    Lemma simul_pure_head_stepₛ eₜ eₛ1 eₛ2 Φ :
+      pure_head_step eₛ1 eₛ2 →
+      SIM eₜ ≲ eₛ2 {{ Φ }} -∗
+      SIM eₜ ≲ eₛ1 {{ Φ }}.
+    Proof.
+      iIntros. iApply simul_pure_stepₛ; eauto using pure_head_step_pure_step.
+    Qed.
+    Lemma simul_pure_head_execₛ ϕ n eₜ eₛ1 eₛ2 Φ :
+      PureHeadExec ϕ n eₛ1 eₛ2 →
+      ϕ →
+      SIM eₜ ≲ eₛ2 {{ Φ }} -∗
+      SIM eₜ ≲ eₛ1 {{ Φ }}.
+    Proof.
+      iIntros. iApply simul_pure_execₛ; eauto using pure_head_exec_pure_exec.
+    Qed.
+  End ectx_lang.
+End bi.
+
+From iris.base_logic.lib Require Import
+  iprop.
+
+Section adequacy.
+  Context {Σ : gFunctors}.
+  Let PROP := iPropI Σ.
+  Context `{SimulGS PROP Λₜ Λₛ}.
+  Context `{Similar (val Λₜ) (val Λₛ)}.
+  Context `{BiSimilar PROP (val Λₜ) (val Λₛ)}.
+  Context (val_equiv_adequacy : ∀ vₜ vₛ, vₜ ≈ vₛ -∗ ⌜vₜ ≈ vₛ⌝).
+  Implicit Types P : PROP.
+  Implicit Types eₜ : expr Λₜ.
+  Implicit Types eₛ : expr Λₛ.
+  Implicit Types σₜ : state Λₜ.
+  Implicit Types σₛ : state Λₛ.
+
+  Definition sat P :=
+    ∃ x, ✓{0} x ∧ uPred_holds P 0 x.
+
+  Lemma sat_intro P :
+    (⊢ P) → sat P.
+  Proof.
+    intros HP. exists ε. split; first by apply ucmra_unit_validN.
+    apply HP; first by apply ucmra_unit_validN.
+    uPred.unseal. done.
+  Qed.
+
+  Lemma sat_elim ϕ :
+    sat ⌜ϕ⌝ → ϕ.
+  Proof.
+    rewrite /sat. uPred.unseal. intros (x & _ & Hϕ). apply Hϕ.
+  Qed.
+
+  Lemma simul_adequacy eₜ σₜ eₛ σₛ :
+    (⊢@{PROP} SIM eₜ ≲ eₛ {{ simul_post_val }} ∗ simul_state_interp σₜ σₛ) →
+    (eₜ, σₜ) ⊴ (eₛ, σₛ).
+  Proof.
+    intros Hiris. apply sat_elim, sat_intro.
+    iDestruct Hiris as "(? & ?)". iApply simul_refinement; eauto.
+  Qed.
+End adequacy.
