theories/without_calls/tmc/lang/ectx_decompositions.v
@@ -1,0 +1,100 @@
+From stdpp Require Import
+  list.
+
+From simuliris.common Require Import
+  prelude
+  tactics.
+From simuliris.without_calls.tmc Require Export
+  lang.lang.
+
+Fixpoint ectx_decompositions e :=
+  let ectx_decompositions_with k e :=
+    (λ '(K, e), ([k] ⋅ K, e)) <$> ectx_decompositions e
+  in
+  ([], e) ::
+  match e with
+  | Var _
+  | Val _
+  | Fail
+  | Pair _ _
+  | PairDet _ _ =>
+      []
+  | Let e1 e2 =>
+      ectx_decompositions_with (EctxLet e2) e1
+  | Match e0 e1 e2 =>
+      ectx_decompositions_with (EctxMatch e1 e2) e0
+  | Store e1 e2 e3 =>
+      ectx_decompositions_with (EctxStore1 e2 e3) e1 ++
+      match to_val e1 with
+      | None =>
+          []
+      | Some v1 =>
+          ectx_decompositions_with (EctxStore2 v1 e3) e2 ++
+          match to_val e2 with
+          | None =>
+              []
+          | Some v2 =>
+              ectx_decompositions_with (EctxStore3 v1 v2) e3
+          end
+      end
+  end.
+
+Lemma ectx_decompositions_sound e K e' :
+  (K, e') ∈ ectx_decompositions e →
+  e = K @@ e'.
+Proof.
+  revert K e'. induction e; simpl; intros;
+  repeat match goal with
+  | _ =>
+      progress decompose_elem_of_list
+  | H : _ ∈ _ <$> _ |- _ =>
+      eapply elem_of_list_fmap in H; simplify
+  | H : _ ∈ match to_val ?e with None => _ | Some _ => _ end |- _ =>
+      let Heq := fresh "Heq" in
+      destruct (to_val e) eqn:Heq; first eapply of_to_val in Heq
+  end;
+  rewrite -?fill_op; naive_solver.
+Qed.
+
+Lemma ectx_decompositions_base e :
+  (∅, e) ∈ ectx_decompositions e.
+Proof.
+  destruct e; econstructor.
+Qed.
+
+Lemma ectx_decompositions_complete K e :
+  (K, e) ∈ ectx_decompositions $ K @@ e.
+Proof.
+  revert K e.
+  assert (
+    ∀ K e,
+    (reverse K, e) ∈ ectx_decompositions $ (reverse K) @@ e).
+  {
+    intros. induction K as [| k K]; first eapply ectx_decompositions_base.
+    rewrite reverse_cons -fill_op /=. destruct k; simpl;
+    repeat match goal with
+    | |- _ ∈ _ :: _ =>
+        econstructor
+    | |- _ ∈ _ <$> _ =>
+        apply elem_of_list_fmap; by exists (reverse K, e)
+    | |- _ ∈ _ ++ _ =>
+        apply elem_of_app; left
+    | _ =>
+        simpl
+    end.
+  }
+  intros. by rewrite -(reverse_involutive K).
+Qed.
+Lemma ectx_decompositions_complete' e K e' :
+  e = K @@ e' →
+  (K, e') ∈ ectx_decompositions e.
+Proof.
+  intros ->. eapply ectx_decompositions_complete.
+Qed.
+
+Lemma ectx_decompositions_spec e K e' :
+  e = K @@ e' ↔
+  (K, e') ∈ ectx_decompositions e.
+Proof.
+  split; eauto using ectx_decompositions_sound, ectx_decompositions_complete'.
+Qed.
