theories/without_calls/tmc/lang/lang.v
@@ -1,0 +1,46 @@
+From simuliris.common Require Import
+  prelude
+  tactics.
+From simuliris.without_calls Require Export
+  lang.ectxi_lang.
+From simuliris.without_calls.tmc Require Export
+  lang.semantics.
+
+Notation of_val := Val.
+
+Definition to_val e :=
+  match e with
+  | Val v => Some v
+  | _ => None
+  end.
+
+Global Instance ectxi_lang_ctxi_base : LangCtxiBase expr ectxi :=
+  ectxi_fill.
+Lemma tmc_lang_mixin :
+  EctxiLangMixin of_val to_val head_step ectxi.
+Proof.
+  econstructor; last (econstructor; first econstructor).
+  - naive_solver.
+  - intros []; naive_solver.
+  - intros * []; naive_solver.
+  - intros [] ?**; naive_solver.
+  - intros []; naive_solver.
+  - intros [] []; naive_solver.
+  - intros [] * Hstep; invert Hstep; naive_solver.
+Qed.
+
+Canonical tmc_ectxi_lang := Build_ectxi_lang tmc_lang_mixin.
+Canonical tmc_ectx_lang := ectx_lang_of_ectxi_lang tmc_ectxi_lang.
+Canonical tmc_lang := lang_of_ectx_lang tmc_ectx_lang.
+
+Global Instance ctxi_lang_ctxi_base : LangCtxiBase expr ctxi :=
+  ctxi_fill.
+Program Global Instance ctxi_lang_ctxi : LangCtxi tmc_lang ctxi :=
+  Build_LangCtxi _.
+Next Obligation.
+  simpl. econstructor.
+  - intros [] ?**; naive_solver.
+  - intros []; naive_solver.
+Qed.
+Global Instance ctx_lang_ctx : LangCtx tmc_lang ctx :=
+  _.
