theories/without_calls/tmc/lang/notations.v
@@ -1,0 +1,77 @@
+From simuliris.common Require Import
+  prelude.
+From simuliris.without_calls.tmc Require Export
+  lang.syntax.
+
+(* ---------- index ---------- *)
+
+Declare Scope index_scope.
+Delimit Scope index_scope with index.
+Bind Scope index_scope with index.
+
+Notation "𝟙" := one.
+Notation "𝟚" := two.
+
+(* ---------- val ---------- *)
+
+Coercion Block : block >-> val.
+Coercion Index : index >-> val.
+
+Declare Scope val_scope.
+Delimit Scope val_scope with V.
+Bind Scope val_scope with val.
+
+Notation "()" := Unit
+: val_scope.
+
+(* ---------- expr ---------- *)
+
+Coercion Val : val >-> expr.
+
+Declare Scope expr_scope.
+Delimit Scope expr_scope with E.
+Bind Scope expr_scope with expr.
+
+Notation "& x" := (Var x%nat%stdpp)
+( at level 8,
+  format "& x"
+).
+
+Notation "# v" := (Val v%index%V%stdpp)
+( at level 8,
+  format "# v"
+).
+
+Notation "'fail'" := Fail
+: expr_scope.
+
+Notation "( e1 , e2 , .. , en )" := (Pair .. (Pair e1%V%E e2%V%E) .. en%V%E)
+: expr_scope.
+
+Notation "⟨ e1 , e2 ⟩" := (PairDet e1%V%E e2%V%E)
+( format "'[hv' ⟨ e1 ,  e2 ⟩ ']'"
+) : expr_scope.
+
+Notation "'let:' e1 'in' e2" := (Let e1%V%E e2%V%E)
+( at level 200,
+  e1, e2 at level 200,
+  format "'[v' 'let:'  '[' e1 ']'  'in' '/' e2 ']'"
+) : expr_scope.
+
+Notation Seq e1 e2 := (Let e1 e2.[ren (+1)]) (only parsing).
+Notation ECtxSeq e2 := (EctxLet e2.[ren (+1)]) (only parsing).
+Notation "e1 ;; e2" := (Seq e1%V%E e2%V%E)
+( at level 100,
+  e2 at level 200,
+  format "'[v' '[hv' '[' e1 ']'  ;; ']' '/' e2 ']'"
+) : expr_scope.
+
+Notation "'match:' e0 'with' () => e1 | '_' => e2 'end'" := (Match e0%V%E e1%V%E e2%V%E)
+( e0, e1, e2 at level 200,
+  format "'[hv' 'match:'  e0  'with'  '/  ' '[' ()  =>  '/    ' e1 ']'  '/' '[' |  '_'  =>  '/    ' e2 ']'  '/' 'end' ']'"
+) : expr_scope.
+
+Notation "e1 .# e2 '<-' e3" := (Store e1%V%E e2%V%E e3%V%E)
+( at level 80,
+  e2 at level 200
+) : expr_scope.
