theories/without_calls/tmc/lang/semantics.v
@@ -1,0 +1,147 @@
+From stdpp Require Export
+  gmap.
+
+From simuliris.common Require Import
+  prelude.
+From simuliris.without_calls.tmc Require Export
+  lang.notations.
+
+Definition state := gmap loc val.
+
+Global Instance state_eq_dec :
+  EqDecision state.
+Proof.
+  solve_decision.
+Defined.
+Global Instance state_inhabited :
+  Inhabited state.
+Proof.
+  apply _.
+Qed.
+
+Canonical Structure stateO := leibnizO state.
+
+Implicit Types blk : block.
+Implicit Types i : index.
+Implicit Types l : loc.
+Implicit Types v : val.
+Implicit Types vs : val * val.
+Implicit Types e : expr.
+Implicit Types σ : state.
+
+Global Instance block_state_lookup : Lookup block (val * val) state :=
+  λ blk σ,
+    match σ !! (blk, 𝟙), σ !! (blk, 𝟚) with
+    | Some v1, Some v2 => Some (v1, v2)
+    | _, _ => None
+    end.
+Lemma block_state_lookup_None blk σ :
+  σ !! blk = None ↔
+  ∃ i, σ !! (blk, i) = None.
+Proof.
+  rewrite {1}/lookup /block_state_lookup.
+  split; [| intros [[]]];
+    destruct (σ !! (blk, 𝟙)) eqn:?, (σ !! (blk, 𝟚)) eqn:?; naive_solver.
+Qed.
+Lemma block_state_lookup_Some blk σ vs :
+  σ !! blk = Some vs ↔
+  σ !! (blk, 𝟙) = Some vs.1 ∧ σ !! (blk, 𝟚) = Some vs.2.
+Proof.
+  rewrite {1}/lookup /block_state_lookup.
+  destruct vs. split;
+    intros Heq;
+    destruct (σ !! (blk, 𝟙)) eqn:Heq1, (σ !! (blk, 𝟚)) eqn:Heq2;
+    rewrite ?Heq in Heq1, Heq2;
+    naive_solver.
+Qed.
+
+Global Instance block_state_insert : Insert block (val * val) state :=
+  λ blk '(v1, v2) σ,
+    <[(blk, 𝟚) := v2]> $ <[(blk, 𝟙) := v1]> σ.
+
+Global Instance loc_state_elem_of : ElemOf loc state :=
+  λ l σ,
+    is_Some (σ !! l).
+Global Instance block_state_elem_of : ElemOf block state :=
+  λ blk σ,
+    ∃ i, (blk, i) ∈ σ.
+Lemma loc_elem_of_state l σ :
+  l ∈ σ ↔
+  is_Some (σ !! l).
+Proof.
+  done.
+Qed.
+Lemma loc_not_elem_of_state l σ :
+  l ∉ σ ↔
+  σ !! l = None.
+Proof.
+  rewrite eq_None_not_Some. done.
+Qed.
+Lemma block_elem_of_state blk σ :
+  blk ∈ σ ↔
+  ∃ i, (blk, i) ∈ σ.
+Proof.
+  done.
+Qed.
+Lemma block_not_elem_of_state blk σ :
+  blk ∉ σ ↔
+  (blk, 𝟙) ∉ σ ∧ (blk, 𝟚) ∉ σ.
+Proof.
+  rewrite block_elem_of_state. split; [| intros ? [[]]]; naive_solver.
+Qed.
+
+Global Instance block_state_fresh : Fresh block state :=
+  λ σ,
+    fresh $ dom (gset _) σ.
+Lemma fresh_block_not_elem_of_state σ :
+  fresh σ ∉ σ.
+Proof.
+  intros [? ?%elem_of_dom]. eapply block_locset_fresh_spec. eexists. done.
+Qed.
+
+Inductive head_step : expr → state → expr → state → Prop :=
+  | head_step_pair_1 e1 e2 σ :
+      head_step
+        (e1, e2) σ
+        (let: e1 in let: e2.[ren (+1)] in ⟨&1, &0⟩) σ
+  | head_step_pair_2 e1 e2 σ :
+      head_step
+        (e1, e2) σ
+        (let: e2 in let: e1.[ren (+1)] in ⟨&0, &1⟩) σ
+  | head_step_pair_det v1 v2 blk σ σ' :
+      blk ∉ σ →
+      σ' = <[blk := (v1, v2)]> σ →
+      head_step
+        ⟨v1, v2⟩ σ
+        blk σ'
+  | head_step_let v e e' σ :
+      e' = e.[#v/] →
+      head_step
+        (let: v in e) σ
+        e' σ
+  | head_step_match_unit e1 e2 σ :
+      head_step
+        match: () with () => e1 | _ => e2 end σ
+        e1 σ
+  | head_step_match_loc blk vs e1 e2 e2' σ :
+      σ !! blk = Some vs →
+      e2' = e2.[#vs.2, #vs.1/] →
+      head_step
+        match: blk with () => e1 | _ => e2 end σ
+        e2' σ
+  | head_step_store blk i v σ σ' :
+      (blk, i) ∈ σ →
+      σ' = <[(blk, i) := v]> σ →
+      head_step
+        (blk .# i <- v) σ
+        #() σ'.
+
+Lemma head_step_pair_det' v1 v2 σ σ' :
+  let blk : block := fresh σ in
+  σ' = <[blk := (v1, v2)]> σ →
+  head_step
+    ⟨v1, v2⟩ σ
+    blk σ'.
+Proof.
+  eauto using head_step_pair_det, fresh_block_not_elem_of_state.
+Qed.
