theories/without_calls/tmc/lang/syntax.v
@@ -1,0 +1,349 @@
+From stdpp Require Import
+  countable.
+
+From iris.algebra Require Export
+  ofe.
+
+From Autosubst Require Export
+  Autosubst.
+
+From simuliris.common Require Import
+  prelude
+  tactics
+  relations.
+From simuliris.common Require Export
+  typeclasses
+  loc.
+
+(* ---------- val ---------- *)
+
+Inductive val :=
+  | Block : block → val
+  | Index : index → val
+  | Unit : val.
+
+Global Instance val_well_formed : WellFormed val :=
+  λ v,
+    match v with
+    | Block _ => False
+    | _ => True
+    end.
+
+Global Instance val_similar : Similar val val :=
+  λ vₜ vₛ,
+    match vₜ, vₛ with
+    | Block _, Block _ => True
+    | Index iₜ, Index iₛ => iₜ = iₛ
+    | Unit, Unit => True
+    | _, _ => False
+    end.
+
+Global Instance val_eq_dec :
+  EqDecision val.
+Proof.
+  solve_decision.
+Qed.
+Global Instance val_countable :
+  Countable val.
+Proof.
+  apply (
+    inj_countable' (
+      λ v,
+        match v with
+        | Block blk => inl blk
+        | Index i => inr (inl i)
+        | Unit => inr (inr ())
+        end
+    ) (
+      λ v,
+        match v with
+        | inl blk => Block blk
+        | inr (inl i) => Index i
+        | inr (inr ()) => Unit
+        end
+    )
+  ).
+  intros []; auto.
+Qed.
+Global Instance val_inhabited : Inhabited val :=
+  populate (Unit).
+
+Canonical Structure valO := leibnizO val.
+
+(* ---------- expr ---------- *)
+
+Inductive expr :=
+  | Var : var → expr
+  | Val : val → expr
+  | Fail : expr
+  | Pair : expr → expr → expr
+  | PairDet : expr → expr → expr
+  | Let : expr → {bind expr} → expr
+  | Match : expr → expr → {bind 2 of expr} → expr
+  | Store : expr → expr → expr → expr.
+
+Global Instance expr_ids : Ids expr. derive. Defined.
+Global Instance expr_rename : Rename expr. derive. Defined.
+Global Instance expr_subst : Subst expr. derive. Defined.
+Global Instance expr_subst_lemmas : SubstLemmas expr. derive. Qed.
+
+Inductive expr_head :=
+  | HeadVar : var → expr_head
+  | HeadVal : val → expr_head
+  | HeadFail : expr_head
+  | HeadPair : expr_head
+  | HeadPairDet : expr_head
+  | HeadLet : expr_head
+  | HeadMatch : expr_head
+  | HeadStore : expr_head.
+
+Definition expr_split e :=
+  match e with
+  | Var x => (HeadVar x, [])
+  | Val v => (HeadVal v, [])
+  | Fail => (HeadFail, [])
+  | Pair e1 e2 => (HeadPair, [e1 ; e2])
+  | PairDet e1 e2 => (HeadPairDet, [e1 ; e2])
+  | Let e1 e2 => (HeadLet, [e1 ; e2])
+  | Match e0 e1 e2 => (HeadMatch, [e0 ; e1 ; e2])
+  | Store e1 e2 e3 => (HeadStore, [e1 ; e2 ; e3])
+  end.
+
+Global Instance expr_head_well_formed : WellFormed expr_head :=
+  λ hd,
+    match hd with
+    | HeadVal (Block _)
+    | HeadPairDet => False
+    | _ => True
+    end.
+
+Global Instance expr_well_formed : WellFormed expr :=
+  fix wf e :=
+    well_formed (expr_split e).1 ∧
+    match e with
+    | Pair e1 e2 => wf e1 ∧ wf e2
+    | PairDet e1 e2 => wf e1 ∧ wf e2
+    | Let e1 e2 => wf e1 ∧ wf e2
+    | Match e0 e1 e2 => wf e0 ∧ wf e1 ∧ wf e2
+    | Store e1 e2 e3 => wf e1 ∧ wf e2 ∧ wf e3
+    | _ => True
+    end.
+
+Fixpoint expr_closed_at n e :=
+  match e with
+  | Var x =>
+      x < n
+  | Val v =>
+      True
+  | Fail =>
+      True
+  | Pair e1 e2 =>
+      expr_closed_at n e1 ∧
+      expr_closed_at n e2
+  | PairDet e1 e2 =>
+      expr_closed_at n e1 ∧
+      expr_closed_at n e2
+  | Let e1 e2 =>
+      expr_closed_at n e1 ∧
+      expr_closed_at (1 + n) e2
+  | Match e0 e1 e2 =>
+      expr_closed_at n e0 ∧
+      expr_closed_at n e1 ∧
+      expr_closed_at (2 + n) e2
+  | Store e1 e2 e3 =>
+      expr_closed_at n e1 ∧
+      expr_closed_at n e2 ∧
+      expr_closed_at n e3
+  end.
+Global Instance expr_closed : Closed expr :=
+  expr_closed_at 0.
+
+Global Instance expr_eq_dec :
+  EqDecision expr.
+Proof.
+  solve_decision.
+Qed.
+Global Instance expr_countable :
+  Countable expr.
+Proof.
+  apply (
+    inj_countable' (
+      fix enc e :=
+        match e with
+        | Val v => GenLeaf $ inl v
+        | Var x => GenLeaf $ inr $ inl x
+        | Fail => GenLeaf $ inr $ inr ()
+        | Pair e1 e2 => GenNode 0 [enc e1; enc e2]
+        | PairDet e1 e2 => GenNode 1 [enc e1; enc e2]
+        | Let e1 e2 => GenNode 2 [enc e1; enc e2]
+        | Match e0 e1 e2 => GenNode 3 [enc e0; enc e1; enc e2]
+        | Store e1 e2 e3 => GenNode 4 [enc e1; enc e2; enc e3]
+        end
+    ) (
+      fix dec e :=
+        match e with
+        | GenLeaf (inl v) => Val v
+        | GenLeaf (inr (inl x)) => Var x
+        | GenLeaf (inr (inr ())) => Fail
+        | GenNode 0 [e1; e2] => Pair (dec e1) (dec e2)
+        | GenNode 1 [e1; e2] => PairDet (dec e1) (dec e2)
+        | GenNode 2 [e1; e2] => Let (dec e1) (dec e2)
+        | GenNode 3 [e0; e1; e2] => Match (dec e0) (dec e1) (dec e2)
+        | GenNode 4 [e1; e2; e3] => Store (dec e1) (dec e2) (dec e3)
+        | _ => Fail
+        end
+    )
+  ).
+  intros e. induction e; try congruence.
+Qed.
+Global Instance expr_inhabited : Inhabited expr :=
+  populate (Val inhabitant).
+
+Canonical Structure exprO := leibnizO expr.
+
+Inductive subexprdir : expr → expr → Prop :=
+  | subexprdir_pair_1 e1 e2 :
+      subexprdir e1 (Pair e1 e2)
+  | subexprdir_pair_2 e1 e2 :
+      subexprdir e2 (Pair e1 e2)
+  | subexprdir_pair_det_1 e1 e2 :
+      subexprdir e1 (PairDet e1 e2)
+  | subexprdir_pair_det_2 e1 e2 :
+      subexprdir e2 (PairDet e1 e2)
+  | subexprdir_let_1 e1 e2 :
+      subexprdir e1 (Let e1 e2)
+  | subexprdir_let_2 e1 e2 :
+      subexprdir e2 (Let e1 e2)
+  | subexprdir_match_0 e0 e1 e2 :
+      subexprdir e0 (Match e0 e1 e2)
+  | subexprdir_match_1 e0 e1 e2 :
+      subexprdir e1 (Match e0 e1 e2)
+  | subexprdir_match_2 e0 e1 e2 :
+      subexprdir e2 (Match e0 e1 e2)
+  | subexprdir_store_1 e1 e2 e3 :
+      subexprdir e1 (Store e1 e2 e3)
+  | subexprdir_store_2 e1 e2 e3 :
+      subexprdir e2 (Store e1 e2 e3)
+  | subexprdir_store_3 e1 e2 e3 :
+      subexprdir e3 (Store e1 e2 e3).
+Lemma subexprdir_wf :
+  wf subexprdir.
+Proof.
+  intros e. induction e; econstructor; intros e' He'; invert He'; try naive_solver.
+Qed.
+
+Definition subexpr :=
+  tc subexprdir.
+Global Instance expr_sqsubset : SqSubset expr :=
+  subexpr.
+Lemma subexpr_wf :
+  wf (⊏).
+Proof.
+  eauto using tc_wf, subexprdir_wf.
+Qed.
+
+(* ---------- ectxi ---------- *)
+
+Inductive ectxi :=
+  | EctxLet : expr → ectxi
+  | EctxMatch : expr → expr → ectxi
+  | EctxStore1 : expr → expr → ectxi
+  | EctxStore2 : val → expr → ectxi
+  | EctxStore3 : val → val → ectxi.
+
+Global Instance ectxi_fill : Fill ectxi expr :=
+  λ k e,
+    match k with
+    | EctxLet e2 =>
+        Let e e2
+    | EctxMatch e1 e2 =>
+        Match e e1 e2
+    | EctxStore1 e2 e3 =>
+        Store e e2 e3
+    | EctxStore2 v1 e3 =>
+        Store (Val v1) e e3
+    | EctxStore3 v1 v2 =>
+        Store (Val v1) (Val v2) e
+    end.
+
+Definition ectxi_split k :=
+  match k with
+  | EctxLet e2 => (HeadLet, [e2])
+  | EctxMatch e1 e2 => (HeadMatch, [e1 ; e2])
+  | EctxStore1 e2 e3 => (HeadStore, [e2 ; e3])
+  | EctxStore2 v1 e3 => (HeadStore, [Val v1 ; e3])
+  | EctxStore3 v1 v2 => (HeadStore, [Val v1 ; Val v2])
+  end.
+
+Global Instance ectxi_well_formed : WellFormed ectxi :=
+  λ k,
+    let '(hd, es) := ectxi_split k in
+    well_formed hd ∧ Forall well_formed es.
+
+(* ---------- ectx ---------- *)
+
+Notation ectx := (list ectxi).
+
+Global Instance ectx_well_formed : WellFormed ectx :=
+  Forall well_formed.
+
+(* ---------- ctxi ---------- *)
+
+Inductive ctxi :=
+  | CtxPair1 : expr → ctxi
+  | CtxPair2 : expr → ctxi
+  | CtxPairDet1 : expr → ctxi
+  | CtxPairDet2 : expr → ctxi
+  | CtxLet1 : expr → ctxi
+  | CtxLet2 : expr → ctxi
+  | CtxMatch0 : expr → expr → ctxi
+  | CtxMatch1 : expr → expr → ctxi
+  | CtxMatch2 : expr → expr → ctxi
+  | CtxStore1 : expr → expr → ctxi
+  | CtxStore2 : expr → expr → ctxi
+  | CtxStore3 : expr → expr → ctxi.
+
+Global Instance ctxi_fill : Fill ctxi expr :=
+  λ c e,
+    match c with
+    | CtxPair1 e2 => Pair e e2
+    | CtxPair2 e1 => Pair e1 e
+    | CtxPairDet1 e2 => PairDet e e2
+    | CtxPairDet2 e1 => PairDet e1 e
+    | CtxLet1 e2 => Let e e2
+    | CtxLet2 e1 => Let e1 e
+    | CtxMatch0 e1 e2 => Match e e1 e2
+    | CtxMatch1 e0 e2 => Match e0 e e2
+    | CtxMatch2 e0 e1 => Match e0 e1 e
+    | CtxStore1 e2 e3 => Store e e2 e3
+    | CtxStore2 e1 e3 => Store e1 e e3
+    | CtxStore3 e1 e2 => Store e1 e2 e
+    end.
+
+Definition ctxi_split c :=
+  match c with
+  | CtxPair1 e2 => (HeadPair, [e2])
+  | CtxPair2 e1 => (HeadPair, [e1])
+  | CtxPairDet1 e2 => (HeadPairDet, [e2])
+  | CtxPairDet2 e1 => (HeadPairDet, [e1])
+  | CtxLet1 e2 => (HeadLet, [e2])
+  | CtxLet2 e1 => (HeadLet, [e1])
+  | CtxMatch0 e1 e2 => (HeadMatch, [e1 ; e2])
+  | CtxMatch1 e0 e2 => (HeadMatch, [e0 ; e2])
+  | CtxMatch2 e0 e1 => (HeadMatch, [e0 ; e1])
+  | CtxStore1 e2 e3 => (HeadStore, [e2 ; e3])
+  | CtxStore2 e1 e3 => (HeadStore, [e1 ; e3])
+  | CtxStore3 e1 e2 => (HeadStore, [e1 ; e2])
+  end.
+
+Global Instance ctxi_well_formed : WellFormed ctxi :=
+  λ c,
+    let '(hd, es) := ctxi_split c in
+    well_formed hd ∧ Forall well_formed es.
+
+(* ---------- ctx ---------- *)
+
+Notation ctx := (list ctxi).
+
+Global Instance ctx_well_formed : WellFormed ctx :=
+  Forall well_formed.
