theories/without_calls/tmc/lang/tactics.v
@@ -1,0 +1,106 @@
+From simuliris.common Require Import
+  prelude
+  tactics.
+From simuliris.without_calls.tmc Require Export
+  lang.ectx_decompositions.
+
+Ltac invert_head_step :=
+  repeat match goal with
+  | _ =>
+      progress simplify_map_eq/=
+  | H : to_val _ = Some _ |- _ =>
+      apply of_to_val in H
+  | H : head_step ?e _ _ _ |- _ =>
+      try (is_var e; fail 1);
+      invert H
+  end.
+
+Create HintDb tmc_lang.
+
+#[export] Hint Extern 0 (
+  head_reducible _ _
+) => (
+  apply strongly_head_reducible
+) : tmc_lang.
+#[export] Hint Extern 1 (
+  head_reducible _ _
+) => (
+  eexists _, _; simpl
+) : tmc_lang.
+#[export] Hint Extern 0 (
+  head_step (PairDet _ _) _ _ _
+) => (
+  eapply head_step_pair_det'
+) : tmc_lang.
+#[export] Hint Extern 1 (
+  head_step _ _ _ _
+) => (
+  econstructor
+) : tmc_lang.
+
+#[export] Hint Extern 0 (
+  sub_redexes_are_values _
+) => (
+  let Hdecomps := fresh "Hdecomps" in
+  intros ?* Hdecomps%ectx_decompositions_spec; invert Hdecomps; first done;
+    decompose_elem_of_list; simplify
+) : tmc_lang.
+
+#[export] Hint Resolve fresh_block_not_elem_of_state
+: tmc_lang.
+
+Ltac unfold_elem_of_state :=
+  repeat match goal with H : _ |- _ =>
+    first [
+      rewrite loc_not_elem_of_state in H
+    | rewrite block_not_elem_of_state in H
+    | rewrite loc_elem_of_state in H
+    | rewrite block_elem_of_state in H
+    ]
+  end;
+  repeat first [
+    rewrite loc_not_elem_of_state
+  | rewrite block_not_elem_of_state
+  | rewrite loc_elem_of_state
+  | rewrite block_elem_of_state
+  ].
+Ltac unfold_state_lookup :=
+  repeat match goal with H : _ |- _ =>
+    first [
+      rewrite block_state_lookup_None in H
+    | rewrite block_state_lookup_Some in H
+    | rewrite (lookup_insert_None (K := loc) (M := gmap loc) (A := val)) in H
+    | rewrite (lookup_insert_Some (K := loc) (M := gmap loc) (A := val)) in H
+    | rewrite (lookup_delete_None (K := loc) (M := gmap loc) (A := val)) in H
+    | rewrite (lookup_delete_Some (K := loc) (M := gmap loc) (A := val)) in H
+    | rewrite (lookup_difference_None (K := loc) (M := gmap loc) (A := val)) in H
+    | rewrite (lookup_difference_Some (K := loc) (M := gmap loc) (A := val)) in H
+    | rewrite (lookup_intersection_None (K := loc) (M := gmap loc) (A := val)) in H
+    | rewrite (lookup_intersection_Some (K := loc) (M := gmap loc) (A := val)) in H
+    | rewrite (lookup_union_None (K := loc) (M := gmap loc) (A := val)) in H
+    | rewrite (lookup_union_Some (K := loc) (M := gmap loc) (A := val)) in H
+    ]
+  end;
+  repeat first [
+    rewrite block_state_lookup_None
+  | rewrite block_state_lookup_Some
+  | rewrite (lookup_insert_None (K := loc) (M := gmap loc) (A := val))
+  | rewrite (lookup_insert_Some (K := loc) (M := gmap loc) (A := val))
+  | rewrite (lookup_delete_None (K := loc) (M := gmap loc) (A := val))
+  | rewrite (lookup_delete_Some (K := loc) (M := gmap loc) (A := val))
+  | rewrite (lookup_difference_None (K := loc) (M := gmap loc) (A := val))
+  | rewrite (lookup_difference_Some (K := loc) (M := gmap loc) (A := val))
+  | rewrite (lookup_intersection_None (K := loc) (M := gmap loc) (A := val))
+  | rewrite (lookup_intersection_Some (K := loc) (M := gmap loc) (A := val))
+  | rewrite (lookup_union_None (K := loc) (M := gmap loc) (A := val))
+  | rewrite (lookup_union_Some (K := loc) (M := gmap loc) (A := val))
+  ].
+Ltac unfold_state_eqns :=
+  unfold_elem_of_state;
+  unfold_state_lookup;
+  simplify.
+Ltac solve_state_eqn :=
+  unfold_state_eqns;
+  naive_solver.
+#[export] Hint Extern 5 => solve_state_eqn
+: tmc_lang.
