theories/without_calls/tmc/simul/bisubst.v
@@ -1,0 +1,31 @@
+From iris.proofmode Require Import
+  proofmode.
+
+From simuliris.common Require Import
+  prelude.
+From simuliris.without_calls.tmc Require Import
+  simul.simul.
+
+Definition bisubst := var → val * val.
+Notation "Γ .ₜ" := (fst ∘ Γ) (at level 5, format "Γ .ₜ").
+Notation "Γ .ₛ" := (snd ∘ Γ) (at level 5, format "Γ .ₛ").
+Notation "Γ .ₜ#" := (of_val ∘ Γ.ₜ) (at level 5, format "Γ .ₜ#").
+Notation "Γ .ₛ#" := (of_val ∘ Γ.ₛ) (at level 5, format "Γ .ₛ#").
+
+Section tmc_simul_heap.
+  Context `{TmcSimulHeapGS Σ}.
+  Implicit Types Γ : bisubst.
+
+  Global Instance bisubst_bi_well_formed : BiWellFormed _ bisubst := (
+    λ Γ,
+      ∀ x, (Γ x).1 ≈ (Γ x).2
+  )%I.
+
+  Definition ground_bisubst : bisubst :=
+    λ _, ((), ())%V.
+  Lemma ground_bisubst_well_formed :
+    ⊢ bi_well_formed ground_bisubst.
+  Proof.
+    iIntros. done.
+  Qed.
+End tmc_simul_heap.
