theories/without_calls/tmc/simul/csimul.v
@@ -1,0 +1,26 @@
+From simuliris.common Require Import
+  prelude.
+From simuliris.without_calls.tmc Require Export
+  simul.simul
+  simul.bisubst.
+
+Class CSimul (PROP : bi) exprₜ exprₛ :=
+  csimul : (exprₜ → exprₛ → PROP) → exprₜ → exprₛ → PROP.
+Notation "'CSIM' eₜ '≲' eₛ '{{' Φ } }" := (csimul Φ eₜ%V%E eₛ%V%E)
+( at level 70,
+  eₜ, eₛ, Φ at level 200,
+  format "'[hv' 'CSIM'  eₜ  ≲  '/   ' eₛ  '/' {{  '[ ' Φ  ']' } } ']'"
+) : bi_scope.
+
+Section tmc_simul_heap.
+  Context `{TmcSimulHeapGS Σ}.
+  Implicit Types v vₜ vₛ : val.
+  Implicit Types e eₜ eₛ : expr.
+  Implicit Types Γ : bisubst.
+
+  Global Instance tmc_csimul : CSimul _ expr expr := (
+    λ Φ eₜ eₛ,
+      ∀ Γ, bi_well_formed Γ -∗
+      SIM eₜ.[Γ.ₜ#] ≲ eₛ.[Γ.ₛ#] {{ Φ }}
+  )%I.
+End tmc_simul_heap.
