theories/without_calls/tmc/simul/rules.v
@@ -1,0 +1,307 @@
+From iris.proofmode Require Import
+  proofmode.
+
+From simuliris.common Require Import
+  prelude
+  tactics.
+From simuliris.without_calls.tmc Require Export
+  lang.tactics
+  simul.simul.
+
+Implicit Types blk blkₜ blkₛ : block.
+Implicit Types i iₜ iₛ : index.
+Implicit Types v vₜ vₛ : val.
+Implicit Types e eₜ eₛ : expr.
+
+Section strongly_head_reducible.
+  Local Ltac solve :=
+    intros ?**; eauto with tmc_lang.
+
+  Global Instance strongly_head_reducible_pair e1 e2 :
+    StronglyHeadReducible (e1, e2)%E.
+  Proof.
+    solve.
+  Qed.
+  Global Instance strongly_head_reducible_pair_det v1 v2 :
+    StronglyHeadReducible ⟨v1, v2⟩%E.
+  Proof.
+    solve.
+  Qed.
+End strongly_head_reducible.
+
+Section strongly_head_irreducible.
+  Local Ltac solve :=
+    intros ** ?** ?** Hstep; invert Hstep; eauto.
+
+  Global Instance strongly_head_irreducible_fail :
+    StronglyHeadIrreducible fail%E.
+  Proof.
+    solve.
+  Qed.
+  Global Instance strongly_head_irreducible_match_index i e1 e2 :
+    StronglyHeadIrreducible match: i with () => e1 | _ => e2 end%E.
+  Proof.
+    solve.
+  Qed.
+  Global Instance strongly_head_irreducible_store_no_block v1 v2 v3 :
+    ¬ (∃ blk, v1 = Block blk) →
+    StronglyHeadIrreducible (v1 .# v2 <- v3)%E.
+  Proof.
+    solve.
+  Qed.
+  Global Instance strongly_head_irreducible_store_no_index v1 v2 v3 :
+    ¬ (∃ i, v2 = Index i) →
+    StronglyHeadIrreducible (v1 .# v2 <- v3)%E.
+  Proof.
+    solve.
+  Qed.
+End strongly_head_irreducible.
+
+Section strongly_head_stuck.
+  Local Ltac solve :=
+    intros; econstructor;
+    typeclasses eauto with core tmc_lang typeclass_instances.
+
+  Global Instance strongly_head_stuck_fail :
+    StronglyHeadStuck fail%E.
+  Proof.
+    solve.
+  Qed.
+  Global Instance strongly_head_stuck_match_index i e1 e2 :
+    StronglyHeadStuck match: i with () => e1 | _ => e2 end%E.
+  Proof.
+    solve.
+  Qed.
+  Global Instance strongly_head_stuck_store_no_block v1 v2 v3 :
+    ¬ (∃ blk, v1 = Block blk) →
+    StronglyHeadStuck (v1 .# v2 <- v3)%E.
+  Proof.
+    solve.
+  Qed.
+  Global Instance strongly_head_stuck_store_no_index v1 v2 v3 :
+    ¬ (∃ i, v2 = Index i) →
+    StronglyHeadStuck (v1 .# v2 <- v3)%E.
+  Proof.
+    solve.
+  Qed.
+End strongly_head_stuck.
+
+Section pure_exec.
+  Local Ltac solve :=
+    eapply pure_head_exec_pure_exec;
+    intros ?; eapply nsteps_once; econstructor;
+    [ eauto with tmc_lang
+    | intros; invert_head_step; eauto
+    ].
+
+  Global Instance pure_exec_let v e :
+    PureExec True 1 (let: #v in e)%E e.[#v/].
+  Proof.
+    solve.
+  Qed.
+  Global Instance pure_exec_match_unit e1 e2 :
+    PureExec True 1 (Match (Val Unit) e1 e2) e1.
+  Proof.
+    solve.
+  Qed.
+End pure_exec.
+
+Section tmc_simul_heap.
+  Context `{TmcSimulHeapGS Σ}.
+  Implicit Types Φ : expr → expr → iProp Σ.
+
+  (* Lemma simul_letₜ vₜ eₜ eₛ Φ : *)
+  (*   SIM eₜ.[#vₜ/] ≲ eₛ {{ Φ }} -∗ *)
+  (*   SIM let: vₜ in eₜ ≲ eₛ {{ Φ }}. *)
+  (* Proof. *)
+  (*   iIntros. iApply simul_pure_execₜ; done. *)
+  (* Qed. *)
+  (* Lemma simul_letₛ eₜ vₛ eₛ Φ : *)
+  (*   SIM eₜ ≲ eₛ.[#vₛ/] {{ Φ }} -∗ *)
+  (*   SIM eₜ ≲ let: vₛ in eₛ {{ Φ }}. *)
+  (* Proof. *)
+  (*   iIntros. iApply simul_pure_execₛ; done. *)
+  (* Qed. *)
+
+  (* Lemma simul_match_unitₜ eₜ1 eₜ2 eₛ Φ : *)
+  (*   SIM eₜ1 ≲ eₛ {{ Φ }} -∗ *)
+  (*   SIM match: () with () => eₜ1 | _ => eₜ2 end ≲ eₛ {{ Φ }}. *)
+  (* Proof. *)
+  (*   iIntros. iApply simul_pure_execₜ; done. *)
+  (* Qed. *)
+  (* Lemma simul_match_unitₛ eₜ eₛ1 eₛ2 Φ : *)
+  (*   SIM eₜ ≲ eₛ1 {{ Φ }} -∗ *)
+  (*   SIM eₜ ≲ match: () with () => eₛ1 | _ => eₛ2 end {{ Φ }}. *)
+  (* Proof. *)
+  (*   iIntros. iApply simul_pure_execₛ; done. *)
+  (* Qed. *)
+
+  Lemma simul_pairₜ eₜ1 eₜ2 eₛ Φ :
+    SIM let: eₜ1 in let: eₜ2.[ren (+1)] in ⟨&1, &0⟩ ≲ eₛ {{ Φ }} -∗
+    SIM let: eₜ2 in let: eₜ1.[ren (+1)] in ⟨&0, &1⟩ ≲ eₛ {{ Φ }} -∗
+    SIM (eₜ1, eₜ2) ≲ eₛ {{ Φ }}.
+  Proof.
+    iIntros. iApply simul_head_stepₜ. iIntros. iModIntro.
+    iSplit; first eauto with tmc_lang.
+    iIntros. iModIntro. invert_head_step; iFrame.
+  Qed.
+  Lemma simul_pairₛ1 eₜ eₛ1 eₛ2 Φ :
+    SIM eₜ ≲ let: eₛ1 in let: eₛ2.[ren (+1)] in ⟨&1, &0⟩ {{ Φ }} -∗
+    SIM eₜ ≲ (eₛ1, eₛ2) {{ Φ }}.
+  Proof.
+    iIntros. iApply simul_head_stepₛ. iIntros. iModIntro.
+    repeat iExists _. iFrame. iPureIntro. econstructor.
+  Qed.
+  Lemma simul_pairₛ2 eₜ eₛ1 eₛ2 Φ :
+    SIM eₜ ≲ let: eₛ2 in let: eₛ1.[ren (+1)] in ⟨&0, &1⟩ {{ Φ }} -∗
+    SIM eₜ ≲ (eₛ1, eₛ2) {{ Φ }}.
+  Proof.
+    iIntros. iApply simul_head_stepₛ. iIntros. iModIntro.
+    repeat iExists _. iFrame. iPureIntro. econstructor.
+  Qed.
+
+  Lemma simul_pair_detₜ vₜ1 vₜ2 eₛ Φ :
+    (∀ blkₜ, blkₜ ↦ₜ (vₜ1, vₜ2) -∗ SIM blkₜ ≲ eₛ {{ Φ }}) -∗
+    SIM ⟨vₜ1, vₜ2⟩ ≲ eₛ {{ Φ }}.
+  Proof.
+    iIntros "H". iApply simul_head_stepₜ. iIntros. iModIntro.
+    iSplit; first eauto with tmc_lang. iIntros. invert_head_step.
+    iMod (simul_heap_alloc_blockₜ with "[$]") as "(? & ?)"; first done.
+    iModIntro. iFrame. iApply "H". iFrame.
+  Qed.
+  Lemma simul_pair_detₛ eₜ vₛ1 vₛ2 Φ :
+    (∀ blkₛ, blkₛ ↦ₛ (vₛ1, vₛ2) -∗ SIM eₜ ≲ blkₛ {{ Φ }}) -∗
+    SIM eₜ ≲ ⟨vₛ1, vₛ2⟩ {{ Φ }}.
+  Proof.
+    iIntros "H". iApply simul_head_stepₛ. iIntros.
+    set blk := fresh σₛ.
+    iMod (simul_heap_alloc_blockₛ _ _ blk with "[$]") as "(? & ?)".
+    { eauto with tmc_lang. }
+    iModIntro. repeat iExists _. iSplit; first (simpl; eauto with tmc_lang).
+    iFrame. iApply "H". iFrame.
+  Qed.
+
+  Lemma simul_pair_unitₜ1 eₜ eₛ :
+    □ (SIM eₜ ≲ eₛ {{ simul_post_val }}) -∗
+    SIM (eₜ, ())
+      ≲ eₛ
+      {{ λ eₜ' eₛ',
+          ∃ blkₜ vₜ vₛ,
+          ⌜eₜ' = blkₜ⌝ ∗ ⌜eₛ' = vₛ⌝ ∗ blkₜ ↦ₜ (vₜ, ()%V) ∗ vₜ ≈ vₛ
+      }}.
+  Proof.
+    iIntros. iApply simul_pairₜ.
+    - iApply (simul_bind' [EctxLet (let: () in ⟨&1, &0⟩)] ∅).
+      iApply (simul_mono with "[] [$]").
+      iIntros (? ?) "(% & % & -> & -> & ?)".
+      do 2 (iApply simul_pure_execₜ; first done).
+      iApply simul_pair_detₜ. iIntros.
+      iApply simul_post. repeat iExists _. eauto.
+    - iApply simul_pure_execₜ; first done.
+      iEval (asimpl).
+      iApply (simul_bind' [EctxLet ⟨&0, ()⟩] ∅).
+      iApply (simul_mono with "[] [$]").
+      iIntros (? ?) "(% & % & -> & -> & ?)".
+      iApply simul_pure_execₜ; first done.
+      iApply simul_pair_detₜ. iIntros.
+      iApply simul_post. repeat iExists _. eauto.
+  Qed.
+  Lemma simul_pair_unitₜ2 eₜ eₛ :
+    □ (SIM eₜ ≲ eₛ {{ simul_post_val }}) -∗
+    SIM ((), eₜ)
+      ≲ eₛ
+      {{ λ eₜ' eₛ',
+          ∃ blkₜ vₜ vₛ,
+          ⌜eₜ' = blkₜ⌝ ∗ ⌜eₛ' = vₛ⌝ ∗ blkₜ ↦ₜ (()%V, vₜ) ∗ vₜ ≈ vₛ
+      }}.
+  Proof.
+    iIntros. iApply simul_pairₜ.
+    - iApply simul_pure_execₜ; first done.
+      iEval (asimpl).
+      iApply (simul_bind' [EctxLet ⟨(), &0⟩] ∅).
+      iApply (simul_mono with "[] [$]").
+      iIntros (? ?) "(% & % & -> & -> & ?)".
+      iApply simul_pure_execₜ; first done.
+      iApply simul_pair_detₜ. iIntros.
+      iApply simul_post. repeat iExists _. eauto.
+    - iApply (simul_bind' [EctxLet (let: #() in ⟨&0, &1⟩)] ∅).
+      iApply (simul_mono with "[] [$]").
+      iIntros (? ?) "(% & % & -> & -> & ?)".
+      do 2 (iApply simul_pure_execₜ; first done).
+      iApply simul_pair_detₜ. iIntros.
+      iApply simul_post. repeat iExists _. eauto.
+  Qed.
+
+  Lemma simul_match_block blkₜ eₜ1 eₜ2 blkₛ eₛ1 eₛ2 Φ :
+    blkₜ ≈ blkₛ -∗
+    ( ∀ vₜ1 vₜ2 vₛ1 vₛ2,
+      (vₜ1, vₜ2) ≈ (vₛ1, vₛ2) -∗
+      SIM eₜ2.[#vₜ2, #vₜ1/] ≲ eₛ2.[#vₛ2, #vₛ1/] {{ Φ }}
+    ) -∗
+    SIM match: blkₜ with () => eₜ1 | _ => eₜ2 end
+      ≲ match: blkₛ with () => eₛ1 | _ => eₛ2 end
+      {{ Φ }}.
+  Proof.
+    iIntros "#? H". iApply simul_head_step. iIntros. iModIntro.
+    iDestruct (simul_heap_bij_valid_block with "[$] [$]") as
+      ([vₜ1 vₜ2] [vₛ1 vₛ2]) "#(% & % & ? & ?)".
+    unfold_state_eqns.
+    iSplit.
+    { iPureIntro. repeat eexists. unshelve econstructor; [exact (vₜ1, vₜ2) | | done].
+      unfold_state_eqns. done.
+    }
+    iIntros. invert_head_step. unfold_state_eqns.
+    iModIntro. repeat iExists _. iSplit.
+    { iPureIntro. repeat eexists. unshelve econstructor; [exact (vₛ1, vₛ2) | | done].
+      unfold_state_eqns. done.
+    }
+    iFrame. iApply "H". iSplit; done.
+  Qed.
+
+  Lemma simul_storeₜ blkₜ iₜ vₜ eₛ Φ :
+    (blkₜ, iₜ) ↦ₜ- -∗
+    ((blkₜ, iₜ) ↦ₜ vₜ -∗ SIM () ≲ eₛ {{ Φ }}) -∗
+    SIM blkₜ .# iₜ <- vₜ ≲ eₛ {{ Φ }}.
+  Proof.
+    iIntros "(% & Hblkₜ) H". iApply simul_head_stepₜ. iIntros. iModIntro. iSplit.
+    { iDestruct (simul_heap_validₜ with "[$] [$]") as "%". eauto with tmc_lang. }
+    iIntros "* %Hstep". invert Hstep.
+    iMod (simul_heap_updateₜ with "[$] [Hblkₜ]") as "(? & ?)"; first by iExists _.
+    iModIntro. iFrame. iApply "H". done.
+  Qed.
+  Lemma simul_storeₛ eₜ blkₛ iₛ vₛ Φ :
+    (blkₛ, iₛ) ↦ₛ- -∗
+    ((blkₛ, iₛ) ↦ₛ vₛ -∗ SIM eₜ ≲ () {{ Φ }}) -∗
+    SIM eₜ ≲ blkₛ .# iₛ <- vₛ {{ Φ }}.
+  Proof.
+    iIntros "(% & Hblkₛ) H". iApply simul_head_stepₛ. iIntros.
+    iDestruct (simul_heap_validₛ with "[$] [$]") as "%".
+    iMod (simul_heap_updateₛ with "[$] [Hblkₛ]") as "(? & ?)"; first by iExists _.
+    iModIntro. repeat iExists _. iSplit; first (simpl; eauto with tmc_lang).
+    iFrame. iApply "H". done.
+  Qed.
+
+  Lemma simul_store blkₜ vₜ blkₛ vₛ i Φ :
+    (blkₜ, i) ≈ (blkₛ, i) -∗
+    vₜ ≈ vₛ -∗
+    SIM () ≲ () {{ Φ }} -∗
+    SIM blkₜ .# i <- vₜ ≲ blkₛ .# i <- vₛ {{ Φ }}.
+  Proof.
+    iIntros. iApply simul_head_step. iIntros. iModIntro.
+    iDestruct (simul_heap_bij_valid with "[$] [$]") as (vₜ' vₛ') "#(% & % & ?)".
+    iSplit; first eauto with tmc_lang.
+    iIntros. invert_head_step.
+    iMod (simul_heap_bij_update _ _ _ _ vₜ with "[$] [$] [$]"). iModIntro.
+    repeat iExists _. iSplit; first eauto with tmc_lang. iFrame.
+  Qed.
+
+  Lemma simul_heap_bij_insert blkₜ vₜ eₜ blkₛ vₛ eₛ i Φ :
+    ((blkₜ, i) ≈ (blkₛ, i) -∗ SIM eₜ ≲ eₛ {{ Φ }}) -∗
+    (blkₜ, i) ⟷ (blkₛ, i) -∗
+    SIM eₜ ≲ eₛ {{ Φ }}.
+  Proof.
+    iIntros "H ?". iApply simul_update_state_interp. iIntros.
+    iMod (simul_heap_bij_insert with "[$] [$]") as "(? & ?)".
+    iModIntro. iFrame. iApply ("H" with "[$]").
+  Qed.
+End tmc_simul_heap.
