theories/without_calls/tmc/soundness.v
@@ -1,0 +1,73 @@
+From simuliris.common Require Import
+  prelude
+  tactics.
+From simuliris.without_calls Require Export
+  refinement.
+From simuliris.without_calls.tmc Require Import
+  simul.proofmode
+  simul.csimul.
+From simuliris.without_calls.tmc Require Export
+  transformation.
+
+Implicit Types blk blkₜ blkₛ : block.
+Implicit Types i iₜ iₛ : index.
+Implicit Types l lₜ lₛ : loc.
+Implicit Types v vₜ vₛ : val.
+Implicit Types e eₜ eₛ : expr.
+
+Section tmc_simul_heap.
+  Context `{TmcSimulHeapGS Σ}.
+
+  Definition simul_post_dps l eₜ eₛ := (
+    ∃ vₜ vₛ,
+    ⌜eₜ = #()⌝ ∗ ⌜eₛ = vₛ⌝ ∗ l ↦ₜ vₜ ∗ vₜ ≈ vₛ
+  )%I.
+
+  Definition tmc_dir_spec' eₛ eₜ :=
+    well_formed eₛ →
+    ⊢ CSIM eₜ ≲ eₛ {{ simul_post_val }}.
+  Definition tmc_dir_spec eₛ eₜ :=
+    tmc_dir eₛ eₜ →
+    tmc_dir_spec' eₛ eₜ.
+  Definition tmc_dps_spec' blkₜ i eₛ eₜ :=
+    well_formed eₛ →
+    (blkₜ, i) ↦ₜ- -∗
+    CSIM eₜ ≲ eₛ {{ simul_post_dps (blkₜ, i) }}.
+  Definition tmc_dps_spec blkₜ i eₛ eₜ :=
+    tmc_dps blkₜ i eₛ eₜ →
+    tmc_dps_spec' blkₜ i eₛ eₜ.
+  Definition tmc_spec eₛ eₜ :=
+    tmc_dir_spec eₛ eₜ ∧
+    ∀ blkₜ i, tmc_dps_spec blkₜ i eₛ eₜ.
+
+  Lemma tmc_sound' eₛ eₜ :
+    tmc_dir_spec eₛ eₜ.
+  Proof.
+    cut (tmc_spec eₛ eₜ). { rewrite /tmc_spec. naive_solver. }
+    revert eₜ. induction eₛ as [eₛ IHeₛ] using (well_founded_ind subexpr_wf).
+    cut (
+      ( ∀ eₛ eₜ,
+        tmc_dir eₛ eₜ →
+        (∀ eₛ' eₜ', eₛ' ⊏ eₛ → tmc_spec eₛ' eₜ') →
+        tmc_dir_spec' eₛ eₜ
+      ) ∧ (
+        ∀ (dst idx : expr) eₛ eₜ,
+        tmc_dps dst idx eₛ eₜ →
+        (∀ eₛ' eₜ', eₛ' ⊏ eₛ → tmc_spec eₛ' eₜ') →
+        ∃ blkₜ i, dst = blkₜ ∧ idx = i ∧ tmc_dps_spec' blkₜ i eₛ eₜ
+      )
+    ). {
+      rewrite {3}/tmc_spec /tmc_dir_spec /tmc_dps_spec /tmc_dir_spec' /tmc_dps_spec'.
+      naive_solver.
+    }
+    clear eₛ IHeₛ. apply tmc_ind.
+    -
+  Qed.
+End tmc_simul_heap.
+
+Lemma tmc_sound eₜ eₛ :
+  well_formed eₛ →
+  tmc_dir eₛ eₜ →
+  eₜ ⊴ eₛ.
+Proof.
+Qed.
