theories/without_calls/tmc/transformation.v
@@ -1,0 +1,164 @@
+From simuliris.common Require Import
+  prelude
+  tactics.
+From simuliris.without_calls.tmc Require Export
+  lang.lang.
+
+Inductive tmc_dir : expr → expr → Prop :=
+  | tmc_dir_var x :
+      tmc_dir
+        &x
+        &x
+  | tmc_dir_val v :
+      tmc_dir
+        #v
+        #v
+  | tmc_dir_fail :
+      tmc_dir
+        fail
+        fail
+  | tmc_dir_pair eₛ1 eₜ1 eₛ2 eₜ2 :
+      tmc_dir eₛ1 eₜ1 →
+      tmc_dir eₛ2 eₜ2 →
+      tmc_dir
+        (eₛ1, eₛ2)
+        (eₜ1, eₜ2)
+  | tmc_dir_pair_det eₛ1 eₜ1 eₛ2 eₜ2 :
+      tmc_dir eₛ1 eₜ1 →
+      tmc_dir eₛ2 eₜ2 →
+      tmc_dir
+        ⟨eₛ1, eₛ2⟩
+        ⟨eₜ1, eₜ2⟩
+  | tmc_dir_let eₛ1 eₜ1 eₛ2 eₜ2 :
+      tmc_dir eₛ1 eₜ1 →
+      tmc_dir eₛ2 eₜ2 →
+      tmc_dir
+        (let: eₛ1 in eₛ2)
+        (let: eₜ1 in eₜ2)
+  | tmc_dir_match eₛ0 eₜ0 eₛ1 eₜ1 eₛ2 eₜ2 :
+      tmc_dir eₛ0 eₜ0 →
+      tmc_dir eₛ1 eₜ1 →
+      tmc_dir eₛ2 eₜ2 →
+      tmc_dir
+        match: eₛ0 with () => eₛ1 | _ => eₛ2 end
+        match: eₜ0 with () => eₜ1 | _ => eₜ2 end
+  | tmc_dir_store eₛ1 eₜ1 eₛ2 eₜ2 eₛ3 eₜ3 :
+      tmc_dir eₛ1 eₜ1 →
+      tmc_dir eₛ2 eₜ2 →
+      tmc_dir eₛ3 eₜ3 →
+      tmc_dir
+        (eₛ1 .# eₛ2 <- eₛ3)
+        (eₜ1 .# eₜ2 <- eₜ3)
+  | tmc_dir_pair_dps_1 eₛ1 eₜ1 eₛ2 eₜ2 :
+      tmc_dir eₛ1 eₜ1 →
+      tmc_dps &0 𝟚 eₛ2.[ren (+1)] eₜ2 →
+      tmc_dir
+        (eₛ1, eₛ2)
+        (let: (eₜ1, ()) in eₜ2 ;; &0)
+  | tmc_dir_pair_dps_2 eₛ1 eₜ1 eₛ2 eₜ2 :
+      tmc_dir eₛ2 eₜ2 →
+      tmc_dps &0 𝟙 eₛ1.[ren (+1)] eₜ1 →
+      tmc_dir
+        (eₛ1, eₛ2)
+        (let: ((), eₜ2) in eₜ1 ;; &0)
+with tmc_dps : expr → expr → expr → expr → Prop :=
+  | tmc_dps_base dst i eₛ eₜ :
+      tmc_dir eₛ eₜ →
+      tmc_dps dst i
+        eₛ
+        (dst .# i <- eₜ)
+  | tmc_dps_fail dst i :
+      tmc_dps dst i
+        fail
+        fail
+  | tmc_dps_pair_1 dst i eₛ1 eₜ1 eₛ2 eₜ2 :
+      tmc_dir eₛ1 eₜ1 →
+      tmc_dps &0 𝟚 eₛ2.[ren (+1)] eₜ2 →
+      tmc_dps dst i
+        (eₛ1, eₛ2)
+        (let: (eₜ1, ()) in dst.[ren (+1)] .# i.[ren (+1)] <- &0 ;; eₜ2)
+  | tmc_dps_pair_2 dst i eₛ1 eₜ1 eₛ2 eₜ2 :
+      tmc_dir eₛ2 eₜ2 →
+      tmc_dps &0 𝟙 eₛ1.[ren (+1)] eₜ1 →
+      tmc_dps dst i
+        (eₛ1, eₛ2)
+        (let: ((), eₜ2) in dst.[ren (+1)] .# i.[ren (+1)] <- &0 ;; eₜ1)
+  | tmc_dps_let dst i eₛ1 eₜ1 eₛ2 eₜ2 :
+      tmc_dir eₛ1 eₜ1 →
+      tmc_dps dst.[ren (+1)] i.[ren (+1)] eₛ2 eₜ2 →
+      tmc_dps dst i
+        (let: eₛ1 in eₛ2)
+        (let: eₜ1 in eₜ2)
+  | tmc_dps_match dst i eₛ0 eₜ0 eₛ1 eₜ1 eₛ2 eₜ2 :
+      tmc_dir eₛ0 eₜ0 →
+      tmc_dps dst i eₛ1 eₜ1 →
+      tmc_dps dst.[ren (+2)] i.[ren (+2)] eₛ2 eₜ2 →
+      tmc_dps dst i
+        match: eₛ0 with () => eₛ1 | _ => eₛ2 end
+        match: eₜ0 with () => eₜ1 | _ => eₜ2 end.
+
+Scheme tmc_dir_dps_ind := Minimality for tmc_dir Sort Prop
+with tmc_dps_dir_ind := Minimality for tmc_dps Sort Prop.
+Combined Scheme tmc_ind from tmc_dir_dps_ind, tmc_dps_dir_ind.
+
+Create HintDb tmc.
+#[export] Hint Constructors tmc_dir : tmc.
+#[export] Hint Constructors tmc_dps : tmc.
+
+Lemma tmc_dir_refl e :
+  tmc_dir e e.
+Proof.
+  induction e; eauto with tmc.
+Qed.
+#[export] Hint Resolve tmc_dir_refl : tmc.
+
+Lemma tmc_subst :
+  ( ∀ eₛ eₜ,
+    tmc_dir eₛ eₜ →
+    ∀ ς, tmc_dir eₛ.[ς] eₜ.[ς]
+  ) ∧ (
+    ∀ dst i eₛ eₜ,
+    tmc_dps dst i eₛ eₜ →
+    ∀ ς, tmc_dps dst.[ς] i.[ς] eₛ.[ς] eₜ.[ς]
+  ).
+Proof.
+  apply tmc_ind; eauto with tmc;
+  try (
+    intros * Hdir IHdir Hdps IHdps *;
+    specialize (IHdps $ up ς); rewrite !subst_comp !up_lift1 -!subst_comp in IHdps;
+    asimpl; rewrite -?subst_comp;
+    constructor; auto
+  ).
+  intros * Hdir0 IHdir0 Hdps1 IHdps1 Hdps2 IHdps2 *.
+  specialize (IHdps2 (upn 2 ς)). rewrite !subst_comp !up_liftn -!subst_comp in IHdps2.
+  constructor; auto.
+Qed.
+Lemma tmc_dir_subst ς eₛ eₜ :
+  tmc_dir eₛ eₜ →
+  tmc_dir eₛ.[ς] eₜ.[ς].
+Proof.
+  eauto using (proj1 tmc_subst).
+Qed.
+#[export] Hint Resolve tmc_dir_subst : tmc.
+Lemma tmc_dps_subst ς dst i eₛ eₜ :
+  tmc_dps dst i eₛ eₜ →
+  tmc_dps dst.[ς] i.[ς] eₛ.[ς] eₜ.[ς].
+Proof.
+  eauto using (proj2 tmc_subst).
+Qed.
+#[export] Hint Resolve tmc_dps_subst : tmc.
+
+Lemma tmc_dir_ctxi (c : ctxi) eₛ eₜ :
+  tmc_dir eₛ eₜ →
+  tmc_dir (c @@ eₛ) (c @@ eₜ).
+Proof.
+  destruct c; eauto with tmc.
+Qed.
+#[export] Hint Resolve tmc_dir_ctxi : tmc.
+Lemma tmc_dir_ctx (C : ctx) eₛ eₜ :
+  tmc_dir eₛ eₜ →
+  tmc_dir (C @@ eₛ) (C @@ eₜ).
+Proof.
+  revert eₛ eₜ. induction C; eauto with tmc.
+Qed.
+#[export] Hint Resolve tmc_dir_ctx : tmc.
